Before: cast construction environment

NuDataStructure.thy
@@ -7,20 +7,49 @@ section \<open>Dynamic List\<close>
 
 definition "DynLst T = (Ref \<lbrace> \<nat>[size_t] \<cross_product> \<nat>[size_t] \<cross_product> Pointer \<rbrace> \<^emph> Array T)
     <where> {(a \<R_arr_tail> (len,cap,ptr),addr \<R_arr_tail> data) | a len cap ptr addr data.
-        length data = cap \<and> ptr = addr \<and> len < cap}
-    <up-lift> (\<lambda>x. case x of (a \<R_arr_tail> (len,cap,ptr),addr \<R_arr_tail> data) \<Rightarrow> a \<R_arr_tail> data)"
+        length data = cap \<and> ptr = addr \<and> len \<le> cap}
+    <up-lift> (\<lambda>x. case x of (a \<R_arr_tail> (len,cap,ptr),addr \<R_arr_tail> data) \<Rightarrow> a \<R_arr_tail> take len data)"
 
-lemma "\<^bold>d\<^bold>e\<^bold>s\<^bold>t \<^bold>c\<^bold>a\<^bold>s\<^bold>t a \<R_arr_tail> data \<tycolon> DynLst T
-  \<longmapsto> (\<exists>* addr. (a \<R_arr_tail> (len,length data,addr),addr \<R_arr_tail> data) \<tycolon> Ref \<lbrace> \<nat>[size_t] \<cross_product> \<nat>[size_t] \<cross_product> Pointer \<rbrace> \<^emph> Array T)
-    \<^bold>w\<^bold>i\<^bold>t\<^bold>h len < length data"
-  unfolding DynLst_def Dest_def
-  apply (\<nu>reason)
+lemma Cast_I: "\<^bold>c\<^bold>a\<^bold>s\<^bold>t A \<longmapsto> B \<^bold>w\<^bold>i\<^bold>t\<^bold>h P \<Longrightarrow> \<^bold>p\<^bold>r\<^bold>e\<^bold>m\<^bold>i\<^bold>s\<^bold>e (P \<longrightarrow> Q) \<Longrightarrow> \<^bold>c\<^bold>a\<^bold>s\<^bold>t A \<longmapsto> B \<^bold>w\<^bold>i\<^bold>t\<^bold>h Q"
+  unfolding Cast_def Premise_def by simp
+lemma Intro_Cast_I: "\<^bold>c\<^bold>a\<^bold>s\<^bold>t A \<longmapsto> B \<^bold>w\<^bold>i\<^bold>t\<^bold>h P \<Longrightarrow> \<^bold>p\<^bold>r\<^bold>e\<^bold>m\<^bold>i\<^bold>s\<^bold>e (P \<longrightarrow> Q) \<Longrightarrow> \<^bold>i\<^bold>n\<^bold>t\<^bold>r\<^bold>o \<^bold>c\<^bold>a\<^bold>s\<^bold>t A \<longmapsto> B \<^bold>w\<^bold>i\<^bold>t\<^bold>h Q"
+  unfolding Intro_def Cast_def Premise_def by simp
+lemma Dest_Cast_I: "\<^bold>c\<^bold>a\<^bold>s\<^bold>t A \<longmapsto> B \<^bold>w\<^bold>i\<^bold>t\<^bold>h P \<Longrightarrow> \<^bold>p\<^bold>r\<^bold>e\<^bold>m\<^bold>i\<^bold>s\<^bold>e (P \<longrightarrow> Q) \<Longrightarrow> \<^bold>d\<^bold>e\<^bold>s\<^bold>t \<^bold>c\<^bold>a\<^bold>s\<^bold>t A \<longmapsto> B \<^bold>w\<^bold>i\<^bold>t\<^bold>h Q"
+  unfolding Dest_def Cast_def Premise_def by simp
+ML \<open>find_first\<close>
 
-lemma "\<^bold>p\<^bold>r\<^bold>e\<^bold>m\<^bold>i\<^bold>s\<^bold>e length data = cap \<Longrightarrow>
-  \<^bold>i\<^bold>n\<^bold>t\<^bold>r\<^bold>o \<^bold>c\<^bold>a\<^bold>s\<^bold>t (a \<R_arr_tail> (len,cap,ptr),addr \<R_arr_tail> data) \<tycolon> Ref \<lbrace> \<nat>[size_t] \<cross_product> \<nat>[size_t] \<cross_product> Pointer \<rbrace> \<^emph> Array T \<longmapsto> a \<R_arr_tail> data \<tycolon> DynLst T"
-  unfolding DynLst_def Intro_def Premise_def
-  ML_val \<open>#goal @{Isar.goal} |> Thm.prop_of\<close>
-  apply (\<nu>reason)
+lemma "(\<And>x. \<exists>y. y = x)" proof
+
+lemma "\<^bold>c\<^bold>a\<^bold>s\<^bold>t a \<R_arr_tail> l \<tycolon> DynLst T
+  \<longmapsto> (\<exists>* addr buf. (a \<R_arr_tail> (length l,length l + length buf,addr),addr \<R_arr_tail> (l @ buf)) \<tycolon> Ref \<lbrace> \<nat>[size_t] \<cross_product> \<nat>[size_t] \<cross_product> Pointer \<rbrace> \<^emph> Array T)"
+  unfolding DynLst_def Cast_def
+  
+  
+  apply (rule Cast_I)
+  ML_val \<open>
+val ctx = Config.put Pattern.unify_trace_failure true @{context}
+fun RSNX tha (i, thb) = let open Thm in
+  (case Seq.chop 2 (biresolution (SOME ctx) false [(false, tha)] i thb) of
+    ([th], _) => solve_constraints th
+  | ([], _) => raise THM ("RSN: no unifiers", i, [tha, thb])
+  | _ => raise THM ("RSN: multiple unifiers", i, [tha, thb]))
+end
+
+
+val x= RSNX @{thm BBB} (1, #goal @{Isar.goal})
+\<close>
+   apply (\<nu>reason) unfolding Premise_def
+  apply auto
+ML \<open>find_first\<close>
+notepad
+begin
+  assume  A[simplified (no_asm_simp)]: "id ((a,b,c) = (a',b',c')) \<Longrightarrow> P (a,b,c)"
+end
+
+lemma "\<^bold>p\<^bold>r\<^bold>e\<^bold>m\<^bold>i\<^bold>s\<^bold>e len < length data \<Longrightarrow>
+  \<^bold>c\<^bold>a\<^bold>s\<^bold>t (a \<R_arr_tail> (len,length data,addr),addr \<R_arr_tail> data) \<tycolon> Ref \<lbrace> \<nat>[size_t] \<cross_product> \<nat>[size_t] \<cross_product> Pointer \<rbrace> \<^emph> Array T
+    \<longmapsto> a \<R_arr_tail> take len data \<tycolon> DynLst T"
+  unfolding DynLst_def by (rule Cast_I) \<nu>reason
 
 
 end
