NuSys.thy
@@ -1,13 +1,13 @@
 (* FIX ME: I have tried the best but the sidekick won't work right. Isabelle is not quite flexible in
   outer syntax and it is already the best hack can be given. *)
 theory NuSys
-  imports NuPrime NuLLReps
+  imports NuPrime
   keywords
     "proc" "rec_proc" :: thy_goal_stmt
   and "as" "\<rightarrow>" "\<longmapsto>" "\<leftarrow>" "^" "^*" "cast" "requires" "\<Longleftarrow>" "\<Longleftarrow>'" "$" "var" "always"  "\<medium_left_bracket>" "\<medium_right_bracket>" "i.e." :: quasi_command
   and "\<bullet>" "affirm" "\<nu>have" "\<nu>obtain" "\<Longrightarrow>" "drop_fact" "\<nu>debug" "\<nu>debug'"
           "\<nu>note" (* "\<nu>choose_quick" *) :: prf_decl % "proof"
-  and "\<nu>processor" "\<nu>processor_resolver" :: thy_decl % "ML"
+  and "\<nu>processor" "\<nu>processor_resolver" "\<nu>reasoner" :: thy_decl % "ML"
   and "\<nu>overloads" "\<nu>cast_overloads" :: thy_decl
   and "finish" :: "qed" % "proof"
 abbrevs
@@ -34,8 +34,51 @@ attribute_setup rotated = \<open>Scan.lift (Scan.optional Parse.int 1 -- Scan.op
   (fn (k,j) => Thm.rule_attribute [] (fn _ => Thm.permute_prems j k))\<close>
   \<open>Enhanced version of the Pure.rotated\<close>
 
+subsection \<open>Prelude of the system\<close>
+
 ML_file NuHelp.ML
 ML_file \<open>library/NuSimpCongruence.ML\<close>
+ML_file \<open>library/cost_net.ML\<close>
+
+subsection \<open>\<nu> Reasoner\<close>
+
+definition "\<nu>Intro_Rule x = x"
+definition "\<nu>Elim_Rule x = x"
+
+ML_file \<open>library/reasoner.ML\<close>
+
+\<nu>reasoner "Different A B" -1 = \<open>let open NuHelp in
+  fn _ => fn th =>
+  case try Thm.major_prem_of th
+    of SOME prem =>
+      (case try (dest_monop @{const_name Trueprop} #> dest_binop @{const_name "Different"}) prem
+        of SOME (a,b) =>
+          if Term.aconv (a,b) then Seq.empty else Seq.single (@{thm Different_I} RS th)
+         | _ => Seq.empty)
+     | _ => Seq.empty
+end\<close>
+
+attribute_setup \<nu>intro =
+\<open>(Scan.lift (Parse.int >> ~) >> Nu_Reasoner.attr_add_intro)
+  || (Scan.lift (Args.add |-- (Parse.int >> ~)) >> Nu_Reasoner.attr_add_intro)
+  || (Scan.lift Args.del >> K Nu_Reasoner.attr_del_intro)\<close>
+  \<open>Set introduction rules in \<nu> reasonser.
+  Syntax: \<nu>intro [add] <spur-of-the-rule> || \<nu>intro del\<close>
+
+attribute_setup \<nu>reasoner_elim =
+\<open>(Scan.lift (Parse.int >> ~) >> Nu_Reasoner.attr_add_elim)
+  || (Scan.lift (Args.add |-- (Parse.int >> ~)) >> Nu_Reasoner.attr_add_elim)
+  || (Scan.lift Args.del >> K Nu_Reasoner.attr_del_elim)\<close>
+  \<open>Set elimduction rules in \<nu> reasonser.
+  Syntax: \<nu>reasoner_elim [add] <spur-of-the-rule> || \<nu>elim del\<close>
+
+
+declare conjI[\<nu>intro 1] TrueI[\<nu>intro 10]
+
+(* ML \<open>Nu_Reasoner.reasoners @{context}\<close>
+
+ML \<open>val th = Goal.init @{cprop "Q \<and> True \<and> A"}
+  val th2 = Nu_Reasoner.reason @{context} th\<close> *)
 
 section \<open>Syntax\<close>
 
@@ -86,7 +129,7 @@ consts key_of :: " 'a \<Rightarrow> 'b "
 
 datatype ('a, 'b) object (infixr "\<R_arr_tail>" 60) = object (key_of_obj: 'a) (val_of_obj: 'b) (infixr "\<R_arr_tail>" 60)
 adhoc_overloading key_of key_of_obj and val_of val_of_obj
-declare object.sel[iff]
+declare object.split[split]
 
 lemma object_forall[lrep_exps]: "All P \<longleftrightarrow> (\<forall>a x. P (a \<R_arr_tail> x))" by (metis object.exhaust)
 lemma object_exists[lrep_exps]: "Ex P \<longleftrightarrow> (\<exists>a x. P (a \<R_arr_tail> x))" by (metis object.exhaust)
@@ -138,8 +181,8 @@ translations
   "\<^bold>c\<^bold>a\<^bold>s\<^bold>t A \<longmapsto> B \<^bold>w\<^bold>i\<^bold>t\<^bold>h P' \<^bold>d\<^bold>u\<^bold>a\<^bold>l a' \<tycolon> A' \<longmapsto> B'" == "\<^bold>c\<^bold>a\<^bold>s\<^bold>t A \<longmapsto> B \<^bold>w\<^bold>i\<^bold>t\<^bold>h P' \<^bold>d\<^bold>u\<^bold>a\<^bold>l \<tort_lbrace>a' \<tycolon> A'\<tort_rbrace> \<longmapsto> B'"
   "\<^bold>c\<^bold>a\<^bold>s\<^bold>t A \<longmapsto> B \<^bold>w\<^bold>i\<^bold>t\<^bold>h P' \<^bold>d\<^bold>u\<^bold>a\<^bold>l A' \<longmapsto> b' \<tycolon> B'" == "\<^bold>c\<^bold>a\<^bold>s\<^bold>t A \<longmapsto> B \<^bold>w\<^bold>i\<^bold>t\<^bold>h P' \<^bold>d\<^bold>u\<^bold>a\<^bold>l A' \<longmapsto> \<tort_lbrace>b' \<tycolon> B'\<tort_rbrace>"
 
-lemma cast_id[\<nu>intro0]: "\<^bold>c\<^bold>a\<^bold>s\<^bold>t A \<longmapsto> A" unfolding Cast_def by fast
-lemma cast_dual_id[\<nu>intro0]: "\<^bold>c\<^bold>a\<^bold>s\<^bold>t A \<longmapsto> A \<^bold>d\<^bold>u\<^bold>a\<^bold>l B \<longmapsto> B"
+lemma cast_id[\<nu>intro 1000000]: "\<^bold>c\<^bold>a\<^bold>s\<^bold>t A \<longmapsto> A" unfolding Cast_def by fast
+lemma cast_dual_id[\<nu>intro 1000000]: "\<^bold>c\<^bold>a\<^bold>s\<^bold>t A \<longmapsto> A \<^bold>d\<^bold>u\<^bold>a\<^bold>l B \<longmapsto> B"
   unfolding CastDual_def Intro_def Dest_def by (simp add: cast_id)
 
 
@@ -156,12 +199,12 @@ Actually, to prevent reasoning loop all the `dest cast` must constitute a DAG in
   while `intro cast` is that of construction.
 \<close>
 
-lemma [\<nu>intro']: "\<^bold>i\<^bold>n\<^bold>t\<^bold>r\<^bold>o \<^bold>c\<^bold>a\<^bold>s\<^bold>t B' \<longmapsto> B \<^bold>w\<^bold>i\<^bold>t\<^bold>h Any \<Longrightarrow> \<^bold>c\<^bold>a\<^bold>s\<^bold>t A \<longmapsto> B' \<^bold>w\<^bold>i\<^bold>t\<^bold>h P \<Longrightarrow> \<^bold>c\<^bold>a\<^bold>s\<^bold>t A \<longmapsto> B \<^bold>w\<^bold>i\<^bold>t\<^bold>h P"
+lemma [\<nu>intro 0]: "\<^bold>i\<^bold>n\<^bold>t\<^bold>r\<^bold>o \<^bold>c\<^bold>a\<^bold>s\<^bold>t B' \<longmapsto> B \<^bold>w\<^bold>i\<^bold>t\<^bold>h Any \<Longrightarrow> \<^bold>c\<^bold>a\<^bold>s\<^bold>t A \<longmapsto> B' \<^bold>w\<^bold>i\<^bold>t\<^bold>h P \<Longrightarrow> \<^bold>c\<^bold>a\<^bold>s\<^bold>t A \<longmapsto> B \<^bold>w\<^bold>i\<^bold>t\<^bold>h P"
   unfolding Intro_def Cast_def by auto
-lemma [\<nu>intro']: "\<^bold>d\<^bold>e\<^bold>s\<^bold>t \<^bold>c\<^bold>a\<^bold>s\<^bold>t A \<longmapsto> A' \<^bold>w\<^bold>i\<^bold>t\<^bold>h P1 \<Longrightarrow> (P1 \<Longrightarrow> \<^bold>c\<^bold>a\<^bold>s\<^bold>t A' \<longmapsto> B \<^bold>w\<^bold>i\<^bold>t\<^bold>h P2) \<Longrightarrow> \<^bold>c\<^bold>a\<^bold>s\<^bold>t A \<longmapsto> B \<^bold>w\<^bold>i\<^bold>t\<^bold>h P1 \<and> P2"
+lemma [\<nu>intro 0]: "\<^bold>d\<^bold>e\<^bold>s\<^bold>t \<^bold>c\<^bold>a\<^bold>s\<^bold>t A \<longmapsto> A' \<^bold>w\<^bold>i\<^bold>t\<^bold>h P1 \<Longrightarrow> (P1 \<Longrightarrow> \<^bold>c\<^bold>a\<^bold>s\<^bold>t A' \<longmapsto> B \<^bold>w\<^bold>i\<^bold>t\<^bold>h P2) \<Longrightarrow> \<^bold>c\<^bold>a\<^bold>s\<^bold>t A \<longmapsto> B \<^bold>w\<^bold>i\<^bold>t\<^bold>h P1 \<and> P2"
   unfolding Dest_def Cast_def by auto
 
-lemma [\<nu>intro'']: "\<^bold>c\<^bold>a\<^bold>s\<^bold>t A \<longmapsto> A' \<^bold>w\<^bold>i\<^bold>t\<^bold>h P \<Longrightarrow> \<^bold>c\<^bold>a\<^bold>s\<^bold>t A \<longmapsto> A' \<^bold>w\<^bold>i\<^bold>t\<^bold>h P \<^bold>d\<^bold>u\<^bold>a\<^bold>l C \<longmapsto> C"
+lemma [\<nu>intro -100]: "\<^bold>c\<^bold>a\<^bold>s\<^bold>t A \<longmapsto> A' \<^bold>w\<^bold>i\<^bold>t\<^bold>h P \<Longrightarrow> \<^bold>c\<^bold>a\<^bold>s\<^bold>t A \<longmapsto> A' \<^bold>w\<^bold>i\<^bold>t\<^bold>h P \<^bold>d\<^bold>u\<^bold>a\<^bold>l C \<longmapsto> C"
   unfolding Cast_def CastDual_def Premise_def Dest_def Intro_def by simp
 
 
@@ -173,8 +216,8 @@ lemma CastI[intro]: "Inhabited A \<Longrightarrow> A \<subseteq> B \<Longrightar
   and [intro]: "\<not> Inhabited A \<Longrightarrow> \<^bold>c\<^bold>a\<^bold>s\<^bold>t A \<longmapsto> B \<^bold>w\<^bold>i\<^bold>t\<^bold>h P" unfolding Cast_def Inhabited_def by auto *)
 
 lemma as_\<nu>proc: "\<^bold>p\<^bold>a\<^bold>r\<^bold>a\<^bold>m x' \<Longrightarrow> \<^bold>p\<^bold>r\<^bold>e\<^bold>m\<^bold>i\<^bold>s\<^bold>e x = x' \<Longrightarrow> \<^bold>c\<^bold>a\<^bold>s\<^bold>t x \<tycolon> N \<longmapsto> x' \<tycolon> N" unfolding Cast_def by auto
-lemma [\<nu>intro]: "\<^bold>p\<^bold>r\<^bold>e\<^bold>m\<^bold>i\<^bold>s\<^bold>e x = x' \<Longrightarrow> \<^bold>c\<^bold>a\<^bold>s\<^bold>t x \<tycolon> N \<longmapsto> x' \<tycolon> N" unfolding Cast_def Premise_def by simp
-lemma [\<nu>intro0]: "\<^bold>p\<^bold>r\<^bold>e\<^bold>m\<^bold>i\<^bold>s\<^bold>e x = x" unfolding Premise_def by simp
+lemma [\<nu>intro 100]: "\<^bold>p\<^bold>r\<^bold>e\<^bold>m\<^bold>i\<^bold>s\<^bold>e x = x' \<Longrightarrow> \<^bold>c\<^bold>a\<^bold>s\<^bold>t x \<tycolon> N \<longmapsto> x' \<tycolon> N" unfolding Cast_def Premise_def by simp
+lemma [\<nu>intro 1000000]: "\<^bold>p\<^bold>r\<^bold>e\<^bold>m\<^bold>i\<^bold>s\<^bold>e x = x" unfolding Premise_def by simp
 
 lemma cast_trans: "\<^bold>c\<^bold>a\<^bold>s\<^bold>t A \<longmapsto> B \<^bold>w\<^bold>i\<^bold>t\<^bold>h P \<Longrightarrow> (P \<Longrightarrow> \<^bold>c\<^bold>a\<^bold>s\<^bold>t B \<longmapsto> C \<^bold>w\<^bold>i\<^bold>t\<^bold>h Q) \<Longrightarrow> \<^bold>c\<^bold>a\<^bold>s\<^bold>t A \<longmapsto> C \<^bold>w\<^bold>i\<^bold>t\<^bold>h P \<and> Q"
   unfolding Cast_def by auto
@@ -208,8 +251,7 @@ subsubsection \<open>Auto tag\<close>
 
 definition Auto :: " 'a \<Rightarrow> 'a " where "Auto x = x"
 
-lemma [\<nu>intro']: "\<^bold>i\<^bold>n\<^bold>t\<^bold>r\<^bold>o \<^bold>c\<^bold>a\<^bold>s\<^bold>t x \<tycolon> T \<longmapsto> x \<tycolon> Auto T" unfolding Auto_def Intro_def using cast_id .
-
+lemma [\<nu>intro 1]: "\<^bold>i\<^bold>n\<^bold>t\<^bold>r\<^bold>o \<^bold>c\<^bold>a\<^bold>s\<^bold>t x \<tycolon> T \<longmapsto> x \<tycolon> Auto T" unfolding Auto_def Intro_def using cast_id .
 
 subsubsection \<open>Argument tag\<close>
 
@@ -219,6 +261,97 @@ lemma Argument_I: "P \<Longrightarrow> Argument P" unfolding Argument_def .
 
 text \<open>Sequent in pattern \<^prop>\<open>\<^bold>a\<^bold>r\<^bold>g\<^bold>u\<^bold>m\<^bold>e\<^bold>n\<^bold>t P \<Longrightarrow> PROP Q\<close> hints users to input a theorem \<^prop>\<open>A\<^sub>1 \<Longrightarrow> A\<^sub>n \<Longrightarrow> P\<close>
   in order to deduce the sequent into \<^prop>\<open>A\<^sub>1 \<Longrightarrow> A\<^sub>n \<Longrightarrow> PROP Q\<close>, which is achieved by the `rule` processor.\<close>
+
+
+
+subsection \<open>Case Analysis\<close>
+
+lemma [\<nu>intro 1]: "\<^bold>p\<^bold>r\<^bold>e\<^bold>m\<^bold>i\<^bold>s\<^bold>e A = B x y \<Longrightarrow> \<^bold>p\<^bold>r\<^bold>e\<^bold>m\<^bold>i\<^bold>s\<^bold>e A = case_prod B (x,y)" by simp
+lemma [\<nu>intro 1]: "\<^bold>p\<^bold>r\<^bold>e\<^bold>m\<^bold>i\<^bold>s\<^bold>e A = B x \<Longrightarrow> \<^bold>p\<^bold>r\<^bold>e\<^bold>m\<^bold>i\<^bold>s\<^bold>e A = case_named B (tag x)" by simp
+lemma [\<nu>intro 1]: "\<^bold>p\<^bold>r\<^bold>e\<^bold>m\<^bold>i\<^bold>s\<^bold>e A = B a x \<Longrightarrow> \<^bold>p\<^bold>r\<^bold>e\<^bold>m\<^bold>i\<^bold>s\<^bold>e A = case_object B (a \<R_arr_tail> x)" by simp
+
+definition CaseSplit :: "bool \<Rightarrow> bool" where "CaseSplit x = x"
+lemma [elim!]: "CaseSplit x \<Longrightarrow> (x \<Longrightarrow> C) \<Longrightarrow> C" unfolding CaseSplit_def .
+
+ lemma [elim!]:
+  "y = case_prod f x \<Longrightarrow> (\<And>x1 x2. y = f x1 x2 \<Longrightarrow> C (x1,x2)) \<Longrightarrow> C x"
+  unfolding CaseSplit_def by (cases x) simp
+lemma [elim!]:
+  "y = (case x of a \<R_arr_tail> b \<Rightarrow> f a b) \<Longrightarrow> (\<And>a b. y = f a b \<Longrightarrow> C (a \<R_arr_tail> b)) \<Longrightarrow> C x"
+  unfolding CaseSplit_def by (cases x) simp
+lemma [elim!]:
+  "y = (case x of tag a \<Rightarrow> f a) \<Longrightarrow> (\<And>a. y = f a \<Longrightarrow> C (tag a)) \<Longrightarrow> C x"
+  unfolding CaseSplit_def by (cases x) simp
+
+(* lemma [\<nu>reasoner_elim 10002]:
+  "CaseSplit (y = case_prod f x) \<Longrightarrow> (\<And>x1 x2. CaseSplit (y = f x1 x2) \<Longrightarrow> C (x1,x2)) \<Longrightarrow> C x"
+  unfolding CaseSplit_def by (cases x) simp
+lemma [\<nu>reasoner_elim 10002]:
+  "CaseSplit (y = (case x of a \<R_arr_tail> b \<Rightarrow> f a b)) \<Longrightarrow> (\<And>a b. CaseSplit (y = f a b) \<Longrightarrow> C (a \<R_arr_tail> b)) \<Longrightarrow> C x"
+  unfolding CaseSplit_def by (cases x) simp
+lemma [\<nu>reasoner_elim 10002]:
+  "CaseSplit (y = (case x of tag a \<Rightarrow> f a)) \<Longrightarrow> (\<And>a. CaseSplit (y = f a) \<Longrightarrow> C (tag a)) \<Longrightarrow> C x"
+  unfolding CaseSplit_def by (cases x) simp*)
+
+
+section \<open>Essential Low Models\<close>
+
+class field = lrep \<comment> \<open>a field in the record tuple\<close>
+class field_list = lrep
+
+subsection \<open>Void\<close>
+
+datatype void = void
+declare void.split[split]
+
+lemma [simp]: "x = y" for x :: void by (cases x; cases y) fast
+
+subsubsection \<open>Settings\<close>
+
+instantiation void :: stack begin
+definition llty_void :: "void itself \<Rightarrow> llty" where "llty_void _ = llty_nil"
+definition deepize_void :: "void \<Rightarrow> deep_model" where "deepize_void _ = DM_none"
+instance by standard auto 
+end
+
+instantiation void :: field begin instance by standard end
+instantiation void :: field_list begin instance by standard end
+
+instantiation void :: zero begin
+definition zero_void :: "void" where [simp]: "zero_void = void"
+instance by standard
+end
+
+
+subsubsection \<open>Abstractor\<close>
+
+definition NuVoid :: "(void, unit) \<nu>" where "NuVoid _ = UNIV"
+text \<open>The name `void` coincides that, when a procedure has no input arguments,
+  the \<nu>-type for the input would exactly be @{term Void}. \<close>
+
+consts Void_sugar :: " 'a_sugar " ("Void")
+translations "Void" == "() \<tycolon> CONST NuVoid"
+
+lemma [simp]: "p \<nuLinkL> NuVoid \<nuLinkR> x" unfolding NuVoid_def Refining_def by simp
+lemma [elim!, \<nu>elim]: "Inhabited \<tort_lbrace>Void\<tort_rbrace> \<Longrightarrow> C \<Longrightarrow> C" by simp
+(*translations "a" <= "a \<^bold>a\<^bold>n\<^bold>d CONST Void"*)
+
+subsection \<open>Prod & the pair abstract structure\<close>
+
+instantiation prod :: (field, field_list) field_list begin instance by standard end
+
+instantiation prod :: (zero, zero) zero begin
+definition zero_prod :: "'a \<times> 'b" where [simp]: "zero_prod = (0,0)"
+instance by standard
+end
+instantiation prod :: (ceq, ceq) ceq begin
+definition ceqable_prod :: "heap \<Rightarrow> 'a \<times> 'b \<Rightarrow> 'a \<times> 'b \<Rightarrow> bool" where "ceqable_prod heap = ceqable heap \<times>\<^sub>r ceqable heap"
+lemma [simp]: "ceqable heap (a1,b1) (a2,b2) \<longleftrightarrow> ceqable heap a1 a2 \<and> ceqable heap b1 b2" unfolding ceqable_prod_def by auto
+definition ceq_prod :: "'a \<times> 'b \<Rightarrow> 'a \<times> 'b \<Rightarrow> bool" where "ceq_prod = ceq \<times>\<^sub>r ceq"
+lemma [simp]: "ceq (a1,b1) (a2,b2) \<longleftrightarrow> ceq a1 a2 \<and> ceq b1 b2" unfolding ceq_prod_def by auto
+instance by standard (auto intro: ceq_trans)
+end
+
 
 section \<open>Essential \<nu>-abstractor\<close>
 
@@ -318,7 +451,7 @@ lemma NuTopCtx_cong: "\<tort_lbrace>h \<tycolon> H\<tort_rbrace> \<equiv> \<tort
   unfolding atomize_eq by (auto 0 3)
 simproc_setup NuTopCtx_cong ("\<tort_lbrace>s \<tycolon> S \<heavy_comma> \<^bold>h\<^bold>e\<^bold>a\<^bold>p h \<tycolon> H\<tort_rbrace>") = \<open>K (NuSimpCong.simproc @{thm NuTopCtx_cong})\<close>
 
-lemma [\<nu>intro]: "\<^bold>c\<^bold>a\<^bold>s\<^bold>t h \<tycolon> H \<longmapsto> h' \<tycolon> H' \<^bold>w\<^bold>i\<^bold>t\<^bold>h Ph \<Longrightarrow>
+lemma [\<nu>intro 1]: "\<^bold>c\<^bold>a\<^bold>s\<^bold>t h \<tycolon> H \<longmapsto> h' \<tycolon> H' \<^bold>w\<^bold>i\<^bold>t\<^bold>h Ph \<Longrightarrow>
   \<^bold>c\<^bold>a\<^bold>s\<^bold>t s \<tycolon> S \<longmapsto> s' \<tycolon> S' \<^bold>w\<^bold>i\<^bold>t\<^bold>h Ps \<Longrightarrow>
   \<^bold>c\<^bold>a\<^bold>s\<^bold>t (s \<tycolon> S\<heavy_comma> \<^bold>h\<^bold>e\<^bold>a\<^bold>p h \<tycolon> H) \<longmapsto> (s' \<tycolon> S'\<heavy_comma> \<^bold>h\<^bold>e\<^bold>a\<^bold>p h' \<tycolon> H') \<^bold>w\<^bold>i\<^bold>t\<^bold>h Ph \<and> Ps"
   unfolding Cast_def by simp blast
@@ -334,10 +467,9 @@ lemma [simp]: "(p1,p2) \<nuLinkL> N \<cross_product> M \<nuLinkR> (x1,x2) \<long
   by (simp add: Fusion_def Refining_def)
 lemma [elim,\<nu>elim]: "(x1,x2) \<ratio> N1 \<cross_product> N2 \<Longrightarrow> (x1 \<ratio> N1 \<Longrightarrow> x2 \<ratio> N2 \<Longrightarrow> C) \<Longrightarrow> C" unfolding Inhabited_def by auto
 
+lemma [\<nu>intro 1]: "\<nu>Zero N z1 \<Longrightarrow> \<nu>Zero M z2 \<Longrightarrow> \<nu>Zero (N \<cross_product> M) (z1,z2)" unfolding \<nu>Zero_def by simp
 
-lemma [\<nu>intro]: "\<nu>Zero N z1 \<Longrightarrow> \<nu>Zero M z2 \<Longrightarrow> \<nu>Zero (N \<cross_product> M) (z1,z2)" unfolding \<nu>Zero_def by simp
-
-lemma [\<nu>intro]: "\<^bold>c\<^bold>a\<^bold>s\<^bold>t x \<tycolon> N \<longmapsto> x' \<tycolon> N' \<^bold>w\<^bold>i\<^bold>t\<^bold>h P1 \<Longrightarrow> \<^bold>c\<^bold>a\<^bold>s\<^bold>t y \<tycolon> M \<longmapsto> y' \<tycolon> M' \<^bold>w\<^bold>i\<^bold>t\<^bold>h P2 \<Longrightarrow>
+lemma [\<nu>intro 1]: "\<^bold>c\<^bold>a\<^bold>s\<^bold>t x \<tycolon> N \<longmapsto> x' \<tycolon> N' \<^bold>w\<^bold>i\<^bold>t\<^bold>h P1 \<Longrightarrow> \<^bold>c\<^bold>a\<^bold>s\<^bold>t y \<tycolon> M \<longmapsto> y' \<tycolon> M' \<^bold>w\<^bold>i\<^bold>t\<^bold>h P2 \<Longrightarrow>
   \<^bold>c\<^bold>a\<^bold>s\<^bold>t (x,y) \<tycolon> N \<cross_product> M \<longmapsto> (x',y') \<tycolon> N' \<cross_product> M' \<^bold>w\<^bold>i\<^bold>t\<^bold>h P1 \<and> P2" unfolding Cast_def by simp blast
 
 (* no_notation RepSet ("\<tort_lbrace> _ \<tort_rbrace>" [10] )
@@ -355,7 +487,7 @@ translations " a \<tycolon> A\<heavy_comma> b \<tycolon> B " == " (CONST Pair b 
 
 lemma [simp]: "(pa,pb) \<nuLinkL> A <stack-div> B \<nuLinkR> (xa,xb) \<longleftrightarrow> (pa \<nuLinkL> A \<nuLinkR> xa) \<and> (pb \<nuLinkL> B \<nuLinkR> xb)" unfolding Stack_Delimiter_def by simp
 
-lemma [\<nu>intro]: "\<^bold>c\<^bold>a\<^bold>s\<^bold>t a \<tycolon> A \<longmapsto> a' \<tycolon> A' \<^bold>w\<^bold>i\<^bold>t\<^bold>h P1 \<Longrightarrow> (P1 \<Longrightarrow> \<^bold>c\<^bold>a\<^bold>s\<^bold>t b \<tycolon> B \<longmapsto> b' \<tycolon> B' \<^bold>w\<^bold>i\<^bold>t\<^bold>h P2) \<Longrightarrow>
+lemma [\<nu>intro 1]: "\<^bold>c\<^bold>a\<^bold>s\<^bold>t a \<tycolon> A \<longmapsto> a' \<tycolon> A' \<^bold>w\<^bold>i\<^bold>t\<^bold>h P1 \<Longrightarrow> (P1 \<Longrightarrow> \<^bold>c\<^bold>a\<^bold>s\<^bold>t b \<tycolon> B \<longmapsto> b' \<tycolon> B' \<^bold>w\<^bold>i\<^bold>t\<^bold>h P2) \<Longrightarrow>
   \<^bold>c\<^bold>a\<^bold>s\<^bold>t (a \<tycolon> A\<heavy_comma> b \<tycolon> B) \<longmapsto> (a' \<tycolon> A'\<heavy_comma> b' \<tycolon> B') \<^bold>w\<^bold>i\<^bold>t\<^bold>h P1 \<and> P2"
   unfolding Cast_def by simp blast
 
@@ -376,7 +508,7 @@ text \<open>Normally the stack elements are written `before` the heap elements, 
   The \<^term>\<open>Nu_Front_Stack\<close> allows one writes the stack elements `after` the heap, as \<^term>\<open>s1 \<tycolon> S1\<heavy_comma> \<^bold>h\<^bold>e\<^bold>a\<^bold>p h \<tycolon> H \<heavy_comma>^ s2 \<tycolon> S2\<close>.
   Both of the two \<nu>-types specify the same low concretes.
   It is useful when one needs to specify over the whole remaining stack and heap, e.g., theorem `Until` (see later)
-    which requires body to return \<^term>\<open>x \<tycolon> X \<heavy_comma>^ loop_condition \<tycolon> \<bool>\<close> where the \<^term>\<open>x \<tycolon> X\<close> instantiated by caller
+    which requires body to return \<^term>\<open>x \<tycolon> X \<heavy_comma>^ loop_condition \<tycolon> Boolean\<close> where the \<^term>\<open>x \<tycolon> X\<close> instantiated by caller
     specifies all the heap and remaining stack except the leading loop_condition.\<close>
 
 lemma [simp]: "(h,a,s) \<nuLinkL> Nu_Front_Stack A Ctx \<nuLinkR> (ax,hsx) \<longleftrightarrow> (a \<nuLinkL> A \<nuLinkR> ax) \<and> ((h,s) \<nuLinkL> Ctx \<nuLinkR> hsx)"
@@ -387,11 +519,14 @@ lemma Nu_Front_Stack_cong: "\<tort_lbrace>c \<tycolon> Ctx\<tort_rbrace> \<equiv
   unfolding atomize_eq by auto
 simproc_setup Nu_Front_Stack_cong ("\<tort_lbrace>c \<tycolon> Ctx \<heavy_comma>^ x \<tycolon> T\<tort_rbrace>") = \<open>K (NuSimpCong.simproc @{thm Nu_Front_Stack_cong})\<close>
 
-lemma [\<nu>intro]: "\<^bold>c\<^bold>a\<^bold>s\<^bold>t R\<heavy_comma> \<^bold>h\<^bold>e\<^bold>a\<^bold>p H \<longmapsto> c \<tycolon> Ctx \<^bold>w\<^bold>i\<^bold>t\<^bold>h P \<Longrightarrow> \<^bold>i\<^bold>n\<^bold>t\<^bold>r\<^bold>o \<^bold>c\<^bold>a\<^bold>s\<^bold>t R\<heavy_comma> x \<tycolon> X\<heavy_comma> \<^bold>h\<^bold>e\<^bold>a\<^bold>p H \<longmapsto> c \<tycolon> Ctx \<heavy_comma>^ (x \<tycolon> X)"
+lemma [\<nu>intro 1]: "\<^bold>c\<^bold>a\<^bold>s\<^bold>t R\<heavy_comma> \<^bold>h\<^bold>e\<^bold>a\<^bold>p H \<longmapsto> c \<tycolon> Ctx \<^bold>w\<^bold>i\<^bold>t\<^bold>h P \<Longrightarrow> \<^bold>i\<^bold>n\<^bold>t\<^bold>r\<^bold>o \<^bold>c\<^bold>a\<^bold>s\<^bold>t R\<heavy_comma> x \<tycolon> X\<heavy_comma> \<^bold>h\<^bold>e\<^bold>a\<^bold>p H \<longmapsto> c \<tycolon> Ctx \<heavy_comma>^ (x \<tycolon> X)"
   unfolding Intro_def Cast_def by simp
-lemma [\<nu>intro]: "\<^bold>c\<^bold>a\<^bold>s\<^bold>t c \<tycolon> Ctx \<longmapsto> (R\<heavy_comma> \<^bold>h\<^bold>e\<^bold>a\<^bold>p H) \<^bold>w\<^bold>i\<^bold>t\<^bold>h P
+lemma [\<nu>intro 1]: "\<^bold>c\<^bold>a\<^bold>s\<^bold>t c \<tycolon> Ctx \<longmapsto> (R\<heavy_comma> \<^bold>h\<^bold>e\<^bold>a\<^bold>p H) \<^bold>w\<^bold>i\<^bold>t\<^bold>h P
     \<Longrightarrow> \<^bold>d\<^bold>e\<^bold>s\<^bold>t \<^bold>c\<^bold>a\<^bold>s\<^bold>t c \<tycolon> Ctx \<heavy_comma>^ (x \<tycolon> X) \<longmapsto> (R\<heavy_comma> x \<tycolon> X\<heavy_comma> \<^bold>h\<^bold>e\<^bold>a\<^bold>p H) \<^bold>w\<^bold>i\<^bold>t\<^bold>h P"
   unfolding Dest_def Cast_def by simp blast
+lemma [\<nu>intro 1]: "\<^bold>c\<^bold>a\<^bold>s\<^bold>t x \<tycolon> X \<longmapsto> x' \<tycolon> X' \<^bold>w\<^bold>i\<^bold>t\<^bold>h Q \<Longrightarrow> \<^bold>c\<^bold>a\<^bold>s\<^bold>t R\<heavy_comma> \<^bold>h\<^bold>e\<^bold>a\<^bold>p H \<longmapsto> c \<tycolon> Ctx \<^bold>w\<^bold>i\<^bold>t\<^bold>h P
+  \<Longrightarrow> \<^bold>c\<^bold>a\<^bold>s\<^bold>t R\<heavy_comma> x \<tycolon> X\<heavy_comma> \<^bold>h\<^bold>e\<^bold>a\<^bold>p H \<longmapsto> c \<tycolon> Ctx \<heavy_comma>^ (x' \<tycolon> X') \<^bold>w\<^bold>i\<^bold>t\<^bold>h P \<and> Q"
+  unfolding Cast_def by auto
 
 
 
@@ -409,10 +544,10 @@ syntax "_ExNu_print" :: "logic \<Rightarrow> logic \<Rightarrow> logic"
 
 translations "\<exists>* a b. P" \<rightleftharpoons> "\<exists>* a. (\<exists>*b. P)"
   "\<exists>* c. x \<tycolon> T" => "(\<lambda>c. x) \<tycolon> CONST ExNu (\<lambda>c. T)"
-  "\<exists>* c. x \<tycolon> T" <= "(\<lambda>c. x) \<tycolon> CONST ExNu (\<lambda>c''''''. T)" (*TODO: print translation that alpha-convert the c''''' *)
+(*  "\<exists>* c. x \<tycolon> T" <= "(\<lambda>c. x) \<tycolon> CONST ExNu (\<lambda>c''''''. T)" (*TODO: print translation that alpha-convert the c''''' *)
   "\<exists>* c. x c \<tycolon> T" <= "x \<tycolon> CONST ExNu (\<lambda>c. T)"
   "CONST Pair a b" <= "(CONST Pair a) b"
-  "\<exists>* c. x \<tycolon> T c" <= "(\<lambda>c. x) \<tycolon> CONST ExNu T" 
+  "\<exists>* c. x \<tycolon> T c" <= "(\<lambda>c. x) \<tycolon> CONST ExNu T" *)
 
 notation ExNu_sugar (binder "\<exists>\<^sup>\<nu> " 10)
 
@@ -432,8 +567,8 @@ lemma [simp]: "\<tort_lbrace>y \<tycolon> L \<heavy_comma> x \<tycolon> ExNu T\<
 lemma ExTyp_strip: "(\<^bold>c\<^bold>u\<^bold>r\<^bold>r\<^bold>e\<^bold>n\<^bold>t p \<^bold>r\<^bold>e\<^bold>s\<^bold>u\<^bold>l\<^bold>t\<^bold>s \<^bold>i\<^bold>n (x \<tycolon> ExNu T)) \<equiv> (\<exists>c. \<^bold>c\<^bold>u\<^bold>r\<^bold>r\<^bold>e\<^bold>n\<^bold>t p \<^bold>r\<^bold>e\<^bold>s\<^bold>u\<^bold>l\<^bold>t\<^bold>s \<^bold>i\<^bold>n x c \<tycolon> T c)"
   unfolding CurrentConstruction_def by auto
 
-lemma [\<nu>intro]: "\<^bold>i\<^bold>n\<^bold>t\<^bold>r\<^bold>o \<^bold>c\<^bold>a\<^bold>s\<^bold>t x c \<tycolon> T c \<longmapsto> (\<exists>*c. x c \<tycolon> T c)" unfolding Intro_def Cast_def by simp blast
-lemma [\<nu>intro]: "(\<And>c. \<^bold>c\<^bold>a\<^bold>s\<^bold>t x c \<tycolon> T c \<longmapsto> x' c \<tycolon> T' c \<^bold>w\<^bold>i\<^bold>t\<^bold>h P c) \<Longrightarrow> \<^bold>c\<^bold>a\<^bold>s\<^bold>t (\<exists>*c. x c \<tycolon> T c) \<longmapsto> (\<exists>*c. x' c \<tycolon> T' c) \<^bold>w\<^bold>i\<^bold>t\<^bold>h (\<exists>c. P c)"
+lemma [\<nu>intro -20]: "\<^bold>i\<^bold>n\<^bold>t\<^bold>r\<^bold>o \<^bold>c\<^bold>a\<^bold>s\<^bold>t x c \<tycolon> T c \<longmapsto> (\<exists>*c. x c \<tycolon> T c)" unfolding Intro_def Cast_def by simp blast
+lemma [\<nu>intro 3]: "(\<And>c. \<^bold>c\<^bold>a\<^bold>s\<^bold>t x c \<tycolon> T c \<longmapsto> x' \<tycolon> T' \<^bold>w\<^bold>i\<^bold>t\<^bold>h P c) \<Longrightarrow> \<^bold>c\<^bold>a\<^bold>s\<^bold>t (\<exists>*c. x c \<tycolon> T c) \<longmapsto> x' \<tycolon> T' \<^bold>w\<^bold>i\<^bold>t\<^bold>h (\<exists>c. P c)"
   unfolding Cast_def by auto
 
 
@@ -473,7 +608,7 @@ translations "(x \<tycolon> T) \<and>\<^sup>\<nu> P" \<rightleftharpoons> "x \<t
   "(x \<tycolon> T) \<and> P" => "x \<tycolon> (T \<and>\<^sup>\<nu> P)"
 lemma [simp]: "p \<nuLinkL> T \<and>\<^sup>\<nu> P \<nuLinkR> x \<longleftrightarrow> P \<and> (p \<nuLinkL> T \<nuLinkR> x)" unfolding NuAddition_def Refining_def by simp
 
-lemma [\<nu>intro]: "\<^bold>p\<^bold>r\<^bold>e\<^bold>m\<^bold>i\<^bold>s\<^bold>e P \<Longrightarrow> \<^bold>i\<^bold>n\<^bold>t\<^bold>r\<^bold>o \<^bold>c\<^bold>a\<^bold>s\<^bold>t x \<tycolon> T \<longmapsto> (x \<tycolon> T) \<and>\<^sup>\<nu> P" unfolding Intro_def Cast_def Premise_def by simp
+lemma [\<nu>intro 1]: "\<^bold>p\<^bold>r\<^bold>e\<^bold>m\<^bold>i\<^bold>s\<^bold>e P \<Longrightarrow> \<^bold>i\<^bold>n\<^bold>t\<^bold>r\<^bold>o \<^bold>c\<^bold>a\<^bold>s\<^bold>t x \<tycolon> T \<longmapsto> (x \<tycolon> T) \<and>\<^sup>\<nu> P" unfolding Intro_def Cast_def Premise_def by simp
 
 (* lemma [simp]: "\<tort_lbrace> x \<tycolon> T \<and>\<^sup>\<nu> True\<tort_rbrace> = \<tort_lbrace> x \<tycolon> T \<tort_rbrace>" by auto
 lemma [simp]: "\<tort_lbrace>L \<heavy_comma> (x \<tycolon> T) \<and> P\<tort_rbrace> = \<tort_lbrace>(L \<heavy_comma> x \<tycolon> T) \<and> P\<tort_rbrace>" and [simp]: "\<tort_lbrace>(x \<tycolon> T) \<and> P\<heavy_comma> R\<tort_rbrace> = \<tort_lbrace>(x \<tycolon> T\<heavy_comma> R) \<and> P\<tort_rbrace>"
@@ -547,11 +682,20 @@ notation NuRefine (infixl "<where>" 80)
 lemma [simp]: " p \<nuLinkL> N \<nuRefine> P \<nuLinkR> x \<longleftrightarrow> x \<in> P \<and> ( p \<nuLinkL> N \<nuLinkR> x)" unfolding NuRefine_def Refining_def by auto
 lemma [elim,\<nu>elim]: " x \<ratio> N \<nuRefine> P \<Longrightarrow> (x \<in> P \<Longrightarrow> x \<ratio> N \<Longrightarrow> C) \<Longrightarrow> C" unfolding Inhabited_def by auto
 
-lemma [\<nu>intro]: "\<^bold>p\<^bold>r\<^bold>e\<^bold>m\<^bold>i\<^bold>s\<^bold>e x \<in> S \<Longrightarrow> \<^bold>i\<^bold>n\<^bold>t\<^bold>r\<^bold>o \<^bold>c\<^bold>a\<^bold>s\<^bold>t x \<tycolon> M \<longmapsto> x \<tycolon> M <where> S"
+lemma [\<nu>intro 1]: "\<^bold>p\<^bold>r\<^bold>e\<^bold>m\<^bold>i\<^bold>s\<^bold>e x \<in> S \<Longrightarrow> \<^bold>i\<^bold>n\<^bold>t\<^bold>r\<^bold>o \<^bold>c\<^bold>a\<^bold>s\<^bold>t x \<tycolon> M \<longmapsto> x \<tycolon> M <where> S"
   unfolding Intro_def Cast_def by auto
-lemma [\<nu>intro]: "\<^bold>d\<^bold>e\<^bold>s\<^bold>t \<^bold>c\<^bold>a\<^bold>s\<^bold>t x \<tycolon> M <where> S \<longmapsto> x \<tycolon> M \<^bold>w\<^bold>i\<^bold>t\<^bold>h x \<in> S"
+lemma AAA[\<nu>intro 1]: "\<^bold>d\<^bold>e\<^bold>s\<^bold>t \<^bold>c\<^bold>a\<^bold>s\<^bold>t x \<tycolon> M <where> S \<longmapsto> x \<tycolon> M \<^bold>w\<^bold>i\<^bold>t\<^bold>h x \<in> S"
   unfolding Dest_def Cast_def by auto
+lemma [\<nu>intro 1]: "\<^bold>c\<^bold>a\<^bold>s\<^bold>t x \<tycolon> M \<longmapsto> x' \<tycolon> M' \<^bold>w\<^bold>i\<^bold>t\<^bold>h P \<Longrightarrow> \<^bold>p\<^bold>r\<^bold>e\<^bold>m\<^bold>i\<^bold>s\<^bold>e x' \<in> S \<Longrightarrow> \<^bold>c\<^bold>a\<^bold>s\<^bold>t x \<tycolon> M \<longmapsto> x' \<tycolon> M' <where> S \<^bold>w\<^bold>i\<^bold>t\<^bold>h P"
+  unfolding Cast_def by auto
 lemma refine_\<nu>cast: "\<^bold>p\<^bold>a\<^bold>r\<^bold>a\<^bold>m P \<Longrightarrow> \<^bold>p\<^bold>r\<^bold>e\<^bold>m\<^bold>i\<^bold>s\<^bold>e x \<in> P \<Longrightarrow> \<^bold>c\<^bold>a\<^bold>s\<^bold>t x \<tycolon> N \<longmapsto> x \<tycolon> (N <where> P)" unfolding Cast_def by auto
+
+ML \<open>
+val ctx = Proof_Context.set_mode Proof_Context.mode_schematic @{context}
+fun mk_cterm s = Syntax.read_prop ctx s |> Thm.cterm_of ctx
+val th = Goal.init (mk_cterm "(\<And> x. P x \<Longrightarrow> \<^bold>d\<^bold>e\<^bold>s\<^bold>t \<^bold>c\<^bold>a\<^bold>s\<^bold>t x \<tycolon> M <where> S \<longmapsto> ?M' x \<^bold>w\<^bold>i\<^bold>t\<^bold>h ?P x)")
+val th2 = @{thm AAA} RS th
+\<close>
 
 abbreviation AutoRefine (infixl "<auto-where>" 80)
   where "AutoRefine \<equiv> Auto NuRefine"
@@ -564,7 +708,7 @@ lemma NuRefine_to_auto:"\<tort_lbrace>x \<tycolon> T <where> P \<tort_rbrace> = 
 lemma [\<nu>intro]: " \<^bold>c\<^bold>a\<^bold>s\<^bold>t x \<tycolon> N \<longmapsto> y \<tycolon> M \<^bold>w\<^bold>i\<^bold>t\<^bold>h Q \<Longrightarrow> \<^bold>p\<^bold>r\<^bold>e\<^bold>m\<^bold>i\<^bold>s\<^bold>e y \<in> P \<Longrightarrow> \<^bold>c\<^bold>a\<^bold>s\<^bold>t x \<tycolon> N \<longmapsto> y \<tycolon> M <where> P \<^bold>w\<^bold>i\<^bold>t\<^bold>h Q" unfolding Cast_def by auto
 (* lemma [\<nu>cast_overload E]: " \<^bold>c\<^bold>a\<^bold>s\<^bold>t x \<tycolon> (N \<^bold>w\<^bold>h\<^bold>e\<^bold>r\<^bold>e P) \<longmapsto> x \<tycolon> N \<^bold>w\<^bold>i\<^bold>t\<^bold>h x \<in> P" unfolding Cast_def by auto *)
 *)
-lemma [\<nu>intro]: "\<^bold>p\<^bold>r\<^bold>e\<^bold>m\<^bold>i\<^bold>s\<^bold>e z \<in> S \<Longrightarrow> \<nu>Zero N z \<Longrightarrow> \<nu>Zero (N <where> S) z" unfolding \<nu>Zero_def Premise_def by simp
+lemma [\<nu>intro 1]: "\<^bold>p\<^bold>r\<^bold>e\<^bold>m\<^bold>i\<^bold>s\<^bold>e z \<in> S \<Longrightarrow> \<nu>Zero N z \<Longrightarrow> \<nu>Zero (N <where> S) z" unfolding \<nu>Zero_def Premise_def by simp
 lemma "\<nu>Equal (N <where> P) can_eq eq \<longleftrightarrow> \<nu>Equal N (\<lambda>x y. x \<in> P \<and> y \<in> P \<and> can_eq x y) eq"
   unfolding \<nu>Equal_def by auto
 
@@ -587,14 +731,14 @@ lemma DownLift_exp[simp]: " p \<nuLinkL> N <down-lift> g \<nuLinkR> x \<longleft
 lemma [elim,\<nu>elim]: " x \<ratio> N <down-lift> g \<Longrightarrow> ( g x \<ratio> N \<Longrightarrow> C) \<Longrightarrow> C" unfolding Inhabited_def by simp
 
 (* lemma [\<nu>cast_overload E]: " \<^bold>c\<^bold>a\<^bold>s\<^bold>t x \<tycolon> N <down-lift> g \<longmapsto> g x \<tycolon> N" unfolding Cast_def by simp *)
-lemma [\<nu>intro]: "\<^bold>p\<^bold>r\<^bold>e\<^bold>m\<^bold>i\<^bold>s\<^bold>e g x = x' \<Longrightarrow> \<^bold>c\<^bold>a\<^bold>s\<^bold>t x \<tycolon> N <down-lift> g \<longmapsto> x' \<tycolon> N" unfolding Cast_def by auto
+lemma [\<nu>intro 1]: "\<^bold>p\<^bold>r\<^bold>e\<^bold>m\<^bold>i\<^bold>s\<^bold>e g x = x' \<Longrightarrow> \<^bold>c\<^bold>a\<^bold>s\<^bold>t x \<tycolon> N <down-lift> g \<longmapsto> x' \<tycolon> N" unfolding Cast_def by auto
 
-lemma [\<nu>intro]: "\<^bold>p\<^bold>r\<^bold>e\<^bold>m\<^bold>i\<^bold>s\<^bold>e (g y = x) \<Longrightarrow> \<^bold>i\<^bold>n\<^bold>t\<^bold>r\<^bold>o \<^bold>c\<^bold>a\<^bold>s\<^bold>t x \<tycolon> M \<longmapsto> y \<tycolon> M <down-lift> g"
+lemma [\<nu>intro 1]: "\<^bold>p\<^bold>r\<^bold>e\<^bold>m\<^bold>i\<^bold>s\<^bold>e (g y = x) \<Longrightarrow> \<^bold>i\<^bold>n\<^bold>t\<^bold>r\<^bold>o \<^bold>c\<^bold>a\<^bold>s\<^bold>t x \<tycolon> M \<longmapsto> y \<tycolon> M <down-lift> g"
   unfolding Intro_def Cast_def by auto
-lemma [\<nu>intro]: "\<^bold>d\<^bold>e\<^bold>s\<^bold>t \<^bold>c\<^bold>a\<^bold>s\<^bold>t y \<tycolon> M <down-lift> g \<longmapsto> g y \<tycolon> M"
+lemma [\<nu>intro 1]: "\<^bold>d\<^bold>e\<^bold>s\<^bold>t \<^bold>c\<^bold>a\<^bold>s\<^bold>t y \<tycolon> M <down-lift> g \<longmapsto> g y \<tycolon> M"
   unfolding Dest_def Cast_def by auto
 
-lemma [\<nu>intro]: " \<^bold>c\<^bold>a\<^bold>s\<^bold>t x \<tycolon> N \<longmapsto> y1 \<tycolon> M \<^bold>w\<^bold>i\<^bold>t\<^bold>h P \<Longrightarrow> \<^bold>p\<^bold>r\<^bold>e\<^bold>m\<^bold>i\<^bold>s\<^bold>e y1 = g y  \<Longrightarrow> \<^bold>c\<^bold>a\<^bold>s\<^bold>t x \<tycolon> N \<longmapsto> y \<tycolon> M <down-lift> g" unfolding Cast_def by auto
+lemma [\<nu>intro 1]: " \<^bold>c\<^bold>a\<^bold>s\<^bold>t x \<tycolon> N \<longmapsto> y1 \<tycolon> M \<^bold>w\<^bold>i\<^bold>t\<^bold>h P \<Longrightarrow> \<^bold>p\<^bold>r\<^bold>e\<^bold>m\<^bold>i\<^bold>s\<^bold>e y1 = g y  \<Longrightarrow> \<^bold>c\<^bold>a\<^bold>s\<^bold>t x \<tycolon> N \<longmapsto> y \<tycolon> M <down-lift> g" unfolding Cast_def by auto
 lemma "\<down>lift_\<nu>cast": "\<^bold>p\<^bold>a\<^bold>r\<^bold>a\<^bold>m g \<Longrightarrow> \<^bold>p\<^bold>r\<^bold>e\<^bold>m\<^bold>i\<^bold>s\<^bold>e g y = x \<Longrightarrow> \<^bold>c\<^bold>a\<^bold>s\<^bold>t x \<tycolon> N \<longmapsto> y \<tycolon> N <down-lift> g" unfolding Cast_def by auto
 
 
@@ -621,11 +765,36 @@ lemma [simp]: " p \<nuLinkL> N <up-lift> f \<nuLinkR> x \<longleftrightarrow> (\
   unfolding UpLift_def Refining_def by auto
 lemma [elim,\<nu>elim]: " x \<ratio> N <up-lift> f \<Longrightarrow> (\<And>y. f y = x \<Longrightarrow> y \<ratio> N \<Longrightarrow> C) \<Longrightarrow> C" unfolding Inhabited_def by auto
 
-lemma [\<nu>intro]: "\<^bold>p\<^bold>r\<^bold>e\<^bold>m\<^bold>i\<^bold>s\<^bold>e y = g x \<Longrightarrow> \<^bold>i\<^bold>n\<^bold>t\<^bold>r\<^bold>o \<^bold>c\<^bold>a\<^bold>s\<^bold>t x \<tycolon> M \<longmapsto> y \<tycolon> M <up-lift> g"
+lemma [\<nu>intro 1]: "\<^bold>p\<^bold>r\<^bold>e\<^bold>m\<^bold>i\<^bold>s\<^bold>e y = g x \<Longrightarrow> \<^bold>i\<^bold>n\<^bold>t\<^bold>r\<^bold>o \<^bold>c\<^bold>a\<^bold>s\<^bold>t x \<tycolon> M \<longmapsto> y \<tycolon> M <up-lift> g"
   unfolding Intro_def Cast_def by auto
-lemma [\<nu>intro]: "(\<And> x.  (g x = y) \<Longrightarrow> \<^bold>d\<^bold>e\<^bold>s\<^bold>t \<^bold>c\<^bold>a\<^bold>s\<^bold>t x \<tycolon> M \<longmapsto> N \<^bold>w\<^bold>i\<^bold>t\<^bold>h P) \<Longrightarrow> \<^bold>d\<^bold>e\<^bold>s\<^bold>t \<^bold>c\<^bold>a\<^bold>s\<^bold>t y \<tycolon> M <up-lift> g \<longmapsto> N \<^bold>w\<^bold>i\<^bold>t\<^bold>h P"
-  unfolding Dest_def Cast_def by auto
+lemma [\<nu>intro 2]: "\<^bold>c\<^bold>a\<^bold>s\<^bold>t x \<tycolon> M \<longmapsto> x' \<tycolon> M' \<^bold>w\<^bold>i\<^bold>t\<^bold>h P \<Longrightarrow> \<^bold>p\<^bold>r\<^bold>e\<^bold>m\<^bold>i\<^bold>s\<^bold>e y = g x' \<Longrightarrow> \<^bold>c\<^bold>a\<^bold>s\<^bold>t x \<tycolon> M \<longmapsto> y \<tycolon> M' <up-lift> g"
+  unfolding Cast_def by auto
+(*lemma [\<nu>intro -30]: "(\<And> x. CaseSplit (y = g x) \<Longrightarrow> \<^bold>d\<^bold>e\<^bold>s\<^bold>t \<^bold>c\<^bold>a\<^bold>s\<^bold>t x \<tycolon> M \<longmapsto> N \<^bold>w\<^bold>i\<^bold>t\<^bold>h P) \<Longrightarrow> \<^bold>d\<^bold>e\<^bold>s\<^bold>t \<^bold>c\<^bold>a\<^bold>s\<^bold>t y \<tycolon> M <up-lift> g \<longmapsto> N \<^bold>w\<^bold>i\<^bold>t\<^bold>h P"
+  unfolding Dest_def Cast_def CaseSplit_def by auto *)
+lemma [\<nu>intro -5]: "(\<And> x. y = g x \<Longrightarrow> \<^bold>c\<^bold>a\<^bold>s\<^bold>t x \<tycolon> M \<longmapsto> N \<^bold>w\<^bold>i\<^bold>t\<^bold>h P x) \<Longrightarrow> \<^bold>c\<^bold>a\<^bold>s\<^bold>t y \<tycolon> M <up-lift> g \<longmapsto> N \<^bold>w\<^bold>i\<^bold>t\<^bold>h (\<exists>x. y = g x \<and> P x)"
+  unfolding Dest_def Cast_def CaseSplit_def by auto
+lemma [\<nu>intro 3]: "(\<And> x. y = g x \<Longrightarrow> \<^bold>c\<^bold>a\<^bold>s\<^bold>t x \<tycolon> M \<longmapsto> y' x \<tycolon> M' x \<^bold>w\<^bold>i\<^bold>t\<^bold>h P x) \<Longrightarrow> \<^bold>c\<^bold>a\<^bold>s\<^bold>t y \<tycolon> M <up-lift> g \<longmapsto>( \<exists>*x. y' x \<tycolon> M' x) \<^bold>w\<^bold>i\<^bold>t\<^bold>h (\<exists>x. y = g x \<and> P x)"
+  unfolding Dest_def Cast_def CaseSplit_def by auto
 
+(*term case_prod
+definition Splited_And :: "'y \<Rightarrow> ('x \<Rightarrow> 'y) \<Rightarrow> ('x \<Rightarrow> prop) \<Rightarrow> prop"
+  where "Splited_And y pattern prop \<equiv> (\<And>x. y = pattern x \<Longrightarrow> PROP prop x)"
+
+lemma A: "y = case_prod f x \<Longrightarrow> (\<And>x1 x2. x = (x1,x2) \<Longrightarrow> y = f x1 x2 \<Longrightarrow> C (x1,x2)) \<Longrightarrow> C x" by (cases x) fast
+
+declare [ [ML_print_depth = 200] ]
+ML \<open>Splitter.split_tac\<close>
+ML \<open>
+val th1 = @{thm conjE}
+val th = Goal.init @{cterm "(\<And>x. QQ \<Longrightarrow> y = (case x of (a,b,c) \<Rightarrow> f a b c) \<Longrightarrow> JJ \<Longrightarrow> C x)"}
+val th'2 = REPEAT (eresolve0_tac @{thms A} 1
+  ) th
+  |> Seq.pull
+\<close>
+
+thm if_split
+thm prod.split_asm
+*)
 lemma "\<^bold>d\<^bold>e\<^bold>s\<^bold>t \<^bold>c\<^bold>a\<^bold>s\<^bold>t y \<tycolon> M <up-lift> g \<longmapsto> (\<exists>* x. x \<tycolon> M \<and>\<^sup>\<nu> (g x = y))"
   unfolding Dest_def Cast_def by auto
 
@@ -637,12 +806,6 @@ lemma "\<nu>Equal (N <up-lift> f) can_eq eq \<longleftrightarrow> \<nu>Equal N (
 
 
 section \<open>Mechanisms - II\<close>
-
-subsection \<open>Case Analysis\<close>
-
-lemma [\<nu>intro]: "\<^bold>p\<^bold>r\<^bold>e\<^bold>m\<^bold>i\<^bold>s\<^bold>e A = B x y \<Longrightarrow> \<^bold>p\<^bold>r\<^bold>e\<^bold>m\<^bold>i\<^bold>s\<^bold>e A = case_prod B (x,y)" by simp
-lemma [\<nu>intro]: "\<^bold>p\<^bold>r\<^bold>e\<^bold>m\<^bold>i\<^bold>s\<^bold>e A = B x \<Longrightarrow> \<^bold>p\<^bold>r\<^bold>e\<^bold>m\<^bold>i\<^bold>s\<^bold>e A = case_named B (tag x)" by simp
-lemma [\<nu>intro]: "\<^bold>p\<^bold>r\<^bold>e\<^bold>m\<^bold>i\<^bold>s\<^bold>e A = B a x \<Longrightarrow> \<^bold>p\<^bold>r\<^bold>e\<^bold>m\<^bold>i\<^bold>s\<^bold>e A = case_object B (a \<R_arr_tail> x)" by simp
 
 subsection \<open>Heap\<close>
 
@@ -717,13 +880,13 @@ subsubsection \<open>Cast\<close>
 definition Heap_Cast_Goal :: " (heap, 'x) \<nu> \<Rightarrow> (heap, 'x) \<nu> "  ("\<medium_left_bracket> _ \<medium_right_bracket>") where "Heap_Cast_Goal x = x"
   \<comment> \<open>The protector marks the goal to be gained\<close>
 
-lemma [\<nu>intro0]: "\<^bold>c\<^bold>a\<^bold>s\<^bold>t h \<tycolon> H \<longmapsto> h \<tycolon> \<medium_left_bracket> H \<medium_right_bracket> \<^bold>d\<^bold>u\<^bold>a\<^bold>l h\<^sub>m \<tycolon> \<medium_left_bracket> H\<^sub>m \<medium_right_bracket> \<longmapsto> h\<^sub>m \<tycolon> H\<^sub>m" unfolding Heap_Cast_Goal_def using cast_dual_id .
+lemma [\<nu>intro 1000]: "\<^bold>c\<^bold>a\<^bold>s\<^bold>t h \<tycolon> H \<longmapsto> h \<tycolon> \<medium_left_bracket> H \<medium_right_bracket> \<^bold>d\<^bold>u\<^bold>a\<^bold>l h\<^sub>m \<tycolon> \<medium_left_bracket> H\<^sub>m \<medium_right_bracket> \<longmapsto> h\<^sub>m \<tycolon> H\<^sub>m" unfolding Heap_Cast_Goal_def using cast_dual_id .
 
-lemma context_cast[\<nu>intro]:
+lemma context_cast[\<nu>intro 1]:
   "\<^bold>c\<^bold>a\<^bold>s\<^bold>t k \<tycolon> K \<longmapsto> k' \<tycolon> K' \<^bold>w\<^bold>i\<^bold>t\<^bold>h P \<Longrightarrow> \<^bold>c\<^bold>a\<^bold>s\<^bold>t h \<tycolon> H \<longmapsto> h' \<tycolon> \<medium_left_bracket> H' \<medium_right_bracket> \<^bold>w\<^bold>i\<^bold>t\<^bold>h Q \<Longrightarrow> \<^bold>c\<^bold>a\<^bold>s\<^bold>t (k \<tycolon> K\<heavy_comma> \<^bold>h\<^bold>e\<^bold>a\<^bold>p h \<tycolon> H) \<longmapsto> (k' \<tycolon> K'\<heavy_comma> \<^bold>h\<^bold>e\<^bold>a\<^bold>p h' \<tycolon> H') \<^bold>w\<^bold>i\<^bold>t\<^bold>h P \<and> Q"
   unfolding Cast_def Heap_Cast_Goal_def by (auto simp add: pair_forall)
 
-lemma context_cast_dual[\<nu>intro]:
+lemma context_cast_dual[\<nu>intro 1]:
   "\<^bold>c\<^bold>a\<^bold>s\<^bold>t k \<tycolon> K \<longmapsto> k' \<tycolon> K' \<^bold>w\<^bold>i\<^bold>t\<^bold>h PK
     \<Longrightarrow> (PK \<Longrightarrow> \<^bold>c\<^bold>a\<^bold>s\<^bold>t h \<tycolon> H \<longmapsto> h' \<tycolon> \<medium_left_bracket> H' \<medium_right_bracket> \<^bold>w\<^bold>i\<^bold>t\<^bold>h PH \<^bold>d\<^bold>u\<^bold>a\<^bold>l h2 \<tycolon> \<medium_left_bracket> H2 \<medium_right_bracket> \<longmapsto> h2' \<tycolon> H2')
     \<Longrightarrow> \<^bold>c\<^bold>a\<^bold>s\<^bold>t (k \<tycolon> K\<heavy_comma> \<^bold>h\<^bold>e\<^bold>a\<^bold>p h \<tycolon> H) \<longmapsto> (k' \<tycolon> K'\<heavy_comma> \<^bold>h\<^bold>e\<^bold>a\<^bold>p h' \<tycolon> H') \<^bold>w\<^bold>i\<^bold>t\<^bold>h PK \<and> PH \<^bold>d\<^bold>u\<^bold>a\<^bold>l (k2 \<tycolon> K2\<heavy_comma> \<^bold>h\<^bold>e\<^bold>a\<^bold>p h2 \<tycolon> H2) \<longmapsto> (k2 \<tycolon> K2\<heavy_comma> \<^bold>h\<^bold>e\<^bold>a\<^bold>p h2' \<tycolon> H2')"
@@ -734,32 +897,32 @@ lemma context_cast_dual[\<nu>intro]:
   unfolding Heap_Cast_Goal_def . *)
 (* lemma [\<nu>intro0]: "\<^bold>c\<^bold>a\<^bold>s\<^bold>t A \<longmapsto> A \<^bold>d\<^bold>u\<^bold>a\<^bold>l B \<longmapsto> B" unfolding CastDual_def  by (simp add: cast_id) *)
 
-lemma [\<nu>intro0]: "\<^bold>c\<^bold>a\<^bold>s\<^bold>t L \<heavy_asterisk> h \<tycolon> H \<longmapsto> L \<heavy_asterisk> h \<tycolon> \<medium_left_bracket> H \<medium_right_bracket> \<^bold>d\<^bold>u\<^bold>a\<^bold>l L \<heavy_asterisk> h\<^sub>m \<tycolon> \<medium_left_bracket> H\<^sub>m \<medium_right_bracket> \<longmapsto> L \<heavy_asterisk> h\<^sub>m \<tycolon> H\<^sub>m" unfolding Heap_Cast_Goal_def using cast_dual_id .
+lemma [\<nu>intro 1000]: "\<^bold>c\<^bold>a\<^bold>s\<^bold>t L \<heavy_asterisk> h \<tycolon> H \<longmapsto> L \<heavy_asterisk> h \<tycolon> \<medium_left_bracket> H \<medium_right_bracket> \<^bold>d\<^bold>u\<^bold>a\<^bold>l L \<heavy_asterisk> h\<^sub>m \<tycolon> \<medium_left_bracket> H\<^sub>m \<medium_right_bracket> \<longmapsto> L \<heavy_asterisk> h\<^sub>m \<tycolon> H\<^sub>m" unfolding Heap_Cast_Goal_def using cast_dual_id .
 
-lemma heap_idx_this[\<nu>intro]:
+lemma heap_idx_this[\<nu>intro 4]:
   "\<^bold>c\<^bold>a\<^bold>s\<^bold>t x \<tycolon> X \<longmapsto> Nothing \<heavy_asterisk> x \<tycolon> \<medium_left_bracket> X \<medium_right_bracket> \<^bold>d\<^bold>u\<^bold>a\<^bold>l Nothing \<heavy_asterisk> x\<^sub>m \<tycolon> \<medium_left_bracket> X\<^sub>m \<medium_right_bracket> \<longmapsto> x\<^sub>m \<tycolon> X\<^sub>m"
   unfolding Cast_def Separation_emptyL Heap_Cast_Goal_def CastDual_def Intro_def Dest_def by simp
 
-lemma heap_idx_L[\<nu>intro0]:
+lemma heap_idx_L[\<nu>intro 2]:
   "\<^bold>c\<^bold>a\<^bold>s\<^bold>t h \<tycolon> H \<longmapsto> h' \<tycolon> H' \<heavy_asterisk> x \<tycolon> \<medium_left_bracket> X \<medium_right_bracket> \<^bold>w\<^bold>i\<^bold>t\<^bold>h P \<^bold>d\<^bold>u\<^bold>a\<^bold>l h'\<^sub>m \<tycolon> H'\<^sub>m \<heavy_asterisk> x\<^sub>m \<tycolon> \<medium_left_bracket> X\<^sub>m \<medium_right_bracket> \<longmapsto> h\<^sub>m \<tycolon> H\<^sub>m
     \<Longrightarrow> \<^bold>c\<^bold>a\<^bold>s\<^bold>t l \<tycolon> L \<heavy_asterisk> h \<tycolon> H \<longmapsto> l \<tycolon> L \<heavy_asterisk> h' \<tycolon> H' \<heavy_asterisk> x \<tycolon> \<medium_left_bracket> X \<medium_right_bracket> \<^bold>w\<^bold>i\<^bold>t\<^bold>h P \<^bold>d\<^bold>u\<^bold>a\<^bold>l l \<tycolon> L \<heavy_asterisk> h'\<^sub>m \<tycolon> H'\<^sub>m \<heavy_asterisk> x\<^sub>m \<tycolon> \<medium_left_bracket> X\<^sub>m \<medium_right_bracket> \<longmapsto> l \<tycolon> L \<heavy_asterisk> h\<^sub>m \<tycolon> H\<^sub>m"
   unfolding Cast_def CastDual_def Heap_Cast_Goal_def SepNu_2_SepSet Intro_def Dest_def
   by (smt (verit, del_insts) SeparationSet_assoc SeparationSet_comm SeparationSet_def mem_Collect_eq)
 
-lemma heap_idx_R[\<nu>intro]:
+lemma heap_idx_R[\<nu>intro 1]:
   "\<^bold>c\<^bold>a\<^bold>s\<^bold>t h \<tycolon> H \<longmapsto> h' \<tycolon> H' \<heavy_asterisk> x \<tycolon> \<medium_left_bracket> X \<medium_right_bracket> \<^bold>w\<^bold>i\<^bold>t\<^bold>h P \<^bold>d\<^bold>u\<^bold>a\<^bold>l h'\<^sub>m \<tycolon> H'\<^sub>m \<heavy_asterisk> x\<^sub>m \<tycolon> \<medium_left_bracket> X\<^sub>m \<medium_right_bracket> \<longmapsto> h\<^sub>m \<tycolon> H\<^sub>m
     \<Longrightarrow> \<^bold>c\<^bold>a\<^bold>s\<^bold>t h \<tycolon> H \<heavy_asterisk> r \<tycolon> R \<longmapsto> h' \<tycolon> H' \<heavy_asterisk> r \<tycolon> R \<heavy_asterisk> x \<tycolon> \<medium_left_bracket> X \<medium_right_bracket> \<^bold>w\<^bold>i\<^bold>t\<^bold>h P \<^bold>d\<^bold>u\<^bold>a\<^bold>l h'\<^sub>m \<tycolon> H'\<^sub>m \<heavy_asterisk> r \<tycolon> R \<heavy_asterisk> x\<^sub>m \<tycolon> \<medium_left_bracket> X\<^sub>m \<medium_right_bracket> \<longmapsto> h\<^sub>m \<tycolon> H\<^sub>m \<heavy_asterisk> r \<tycolon> \<medium_left_bracket> R \<medium_right_bracket>"
   unfolding Cast_def CastDual_def Heap_Cast_Goal_def SepNu_2_SepSet Intro_def Dest_def
   by (smt (verit, del_insts) SeparationSet_assoc SeparationSet_comm SeparationSet_def mem_Collect_eq)
 
-lemma [\<nu>intro]:
+lemma [\<nu>intro 0]:
   "\<^bold>c\<^bold>a\<^bold>s\<^bold>t h \<tycolon> H \<longmapsto> h1 \<tycolon> H1 \<heavy_asterisk> x \<tycolon> \<medium_left_bracket> X \<medium_right_bracket> \<^bold>w\<^bold>i\<^bold>t\<^bold>h P1 \<^bold>d\<^bold>u\<^bold>a\<^bold>l h1\<^sub>m \<tycolon> H1\<^sub>m \<heavy_asterisk> x\<^sub>m \<tycolon> \<medium_left_bracket> X\<^sub>m \<medium_right_bracket> \<longmapsto> h\<^sub>m \<tycolon> H\<^sub>m
     \<Longrightarrow> (P1 \<Longrightarrow> \<^bold>c\<^bold>a\<^bold>s\<^bold>t h1 \<tycolon> H1 \<longmapsto> h2 \<tycolon> \<medium_left_bracket> H2 \<medium_right_bracket> \<^bold>w\<^bold>i\<^bold>t\<^bold>h P2 \<^bold>d\<^bold>u\<^bold>a\<^bold>l h2\<^sub>m \<tycolon> \<medium_left_bracket> H2\<^sub>m \<medium_right_bracket> \<longmapsto> h1\<^sub>m \<tycolon> H1\<^sub>m)
     \<Longrightarrow> \<^bold>c\<^bold>a\<^bold>s\<^bold>t h \<tycolon> H \<longmapsto> (x, h2) \<tycolon> \<medium_left_bracket> X <heap-sep> H2 \<medium_right_bracket> \<^bold>w\<^bold>i\<^bold>t\<^bold>h P1 \<and> P2 \<^bold>d\<^bold>u\<^bold>a\<^bold>l (x\<^sub>m, h2\<^sub>m) \<tycolon> \<medium_left_bracket> X\<^sub>m <heap-sep> H2\<^sub>m \<medium_right_bracket> \<longmapsto> h\<^sub>m \<tycolon> H\<^sub>m"
   unfolding Cast_def CastDual_def Heap_Cast_Goal_def SepNu_2_SepSet Intro_def Dest_def
   by (smt (verit, del_insts) SeparationSet_assoc SeparationSet_comm SeparationSet_def mem_Collect_eq)
 
-lemma [ \<nu>intro' ]: "\<^bold>d\<^bold>e\<^bold>s\<^bold>t \<^bold>c\<^bold>a\<^bold>s\<^bold>t x \<tycolon> T \<longmapsto> d \<tycolon> D \<^bold>w\<^bold>i\<^bold>t\<^bold>h P
+lemma [ \<nu>intro -10 ]: "\<^bold>d\<^bold>e\<^bold>s\<^bold>t \<^bold>c\<^bold>a\<^bold>s\<^bold>t x \<tycolon> T \<longmapsto> d \<tycolon> D \<^bold>w\<^bold>i\<^bold>t\<^bold>h P
   \<Longrightarrow> (P \<Longrightarrow> \<^bold>c\<^bold>a\<^bold>s\<^bold>t d \<tycolon> D \<longmapsto> d' \<tycolon> D' \<heavy_asterisk> h \<tycolon> \<medium_left_bracket> H \<medium_right_bracket> \<^bold>w\<^bold>i\<^bold>t\<^bold>h P2 \<^bold>d\<^bold>u\<^bold>a\<^bold>l i'\<^sub>m \<tycolon> I'\<^sub>m \<heavy_asterisk> h\<^sub>m \<tycolon> \<medium_left_bracket> H\<^sub>m \<medium_right_bracket> \<longmapsto> i \<tycolon> I)
   \<Longrightarrow> (P \<Longrightarrow> P2 \<Longrightarrow> \<^bold>i\<^bold>n\<^bold>t\<^bold>r\<^bold>o \<^bold>c\<^bold>a\<^bold>s\<^bold>t i \<tycolon> I \<longmapsto> x\<^sub>m \<tycolon> T \<^bold>w\<^bold>i\<^bold>t\<^bold>h Anyway)
   \<Longrightarrow> \<^bold>c\<^bold>a\<^bold>s\<^bold>t x \<tycolon> T \<longmapsto> d' \<tycolon> D' \<heavy_asterisk> h \<tycolon> \<medium_left_bracket> H \<medium_right_bracket> \<^bold>w\<^bold>i\<^bold>t\<^bold>h P \<and> P2 \<^bold>d\<^bold>u\<^bold>a\<^bold>l i'\<^sub>m \<tycolon> I'\<^sub>m \<heavy_asterisk> h\<^sub>m \<tycolon> \<medium_left_bracket> H\<^sub>m \<medium_right_bracket> \<longmapsto> x\<^sub>m \<tycolon> T"
@@ -832,9 +995,9 @@ definition Conversion :: "('a::lrep \<longmapsto> 'b::lrep) \<Rightarrow> (heap\
 lemma conversion: "\<^bold>c\<^bold>o\<^bold>n\<^bold>v\<^bold>e\<^bold>r\<^bold>s\<^bold>i\<^bold>o\<^bold>n f \<blangle> U \<longmapsto> V \<brangle> \<long_dobule_mapsto> f' \<blangle> U' \<longmapsto> V' \<brangle> \<Longrightarrow> \<^bold>p\<^bold>r\<^bold>o\<^bold>c f \<blangle> U \<longmapsto> V \<brangle> \<Longrightarrow> \<^bold>p\<^bold>r\<^bold>o\<^bold>c f' \<blangle> U' \<longmapsto> V' \<brangle>"
   for f :: " ('a::lrep) \<longmapsto> ('b::lrep)" and f' :: " ('c::lrep) \<longmapsto> ('d::lrep)" unfolding Conversion_def by fast
 
-lemma [\<nu>intro0]: "\<^bold>c\<^bold>o\<^bold>n\<^bold>v\<^bold>e\<^bold>r\<^bold>s\<^bold>i\<^bold>o\<^bold>n f \<blangle> U \<longmapsto> V \<brangle> \<long_dobule_mapsto> f \<blangle> U \<longmapsto> V \<brangle>" unfolding Conversion_def by fast
+lemma [\<nu>intro 1000000]: "\<^bold>c\<^bold>o\<^bold>n\<^bold>v\<^bold>e\<^bold>r\<^bold>s\<^bold>i\<^bold>o\<^bold>n f \<blangle> U \<longmapsto> V \<brangle> \<long_dobule_mapsto> f \<blangle> U \<longmapsto> V \<brangle>" unfolding Conversion_def by fast
 
-lemma conversion_cast[\<nu>intro]: "\<^bold>c\<^bold>a\<^bold>s\<^bold>t U' \<longmapsto> U \<^bold>w\<^bold>i\<^bold>t\<^bold>h P \<^bold>d\<^bold>u\<^bold>a\<^bold>l V \<longmapsto> V' \<Longrightarrow> \<^bold>c\<^bold>o\<^bold>n\<^bold>v\<^bold>e\<^bold>r\<^bold>s\<^bold>i\<^bold>o\<^bold>n f \<blangle> U \<longmapsto> V \<brangle> \<long_dobule_mapsto> f \<blangle> U' \<longmapsto> V'\<brangle>"
+lemma conversion_cast[\<nu>intro 0]: "\<^bold>c\<^bold>a\<^bold>s\<^bold>t U' \<longmapsto> U \<^bold>w\<^bold>i\<^bold>t\<^bold>h P \<^bold>d\<^bold>u\<^bold>a\<^bold>l V \<longmapsto> V' \<Longrightarrow> \<^bold>c\<^bold>o\<^bold>n\<^bold>v\<^bold>e\<^bold>r\<^bold>s\<^bold>i\<^bold>o\<^bold>n f \<blangle> U \<longmapsto> V \<brangle> \<long_dobule_mapsto> f \<blangle> U' \<longmapsto> V'\<brangle>"
   unfolding Conversion_def Procedure_def Cast_def CastDual_def Intro_def Dest_def
   by (metis LooseStateTy_introByStrict LooseStateTy_upgrade StrictStateTy_elim StrictStateTy_intro)
 
@@ -863,12 +1026,12 @@ definition Arguments :: " (heap \<times> 'a) set \<Rightarrow> (heap \<times> 'b
   "Arguments A B R args \<longleftrightarrow> (\<forall>h a. (h,a) \<in> A \<longrightarrow> (h, fst (assemble_arg args a)) \<in> B \<and> snd (assemble_arg args a) \<in> R)
     \<and> (\<forall>h b r. (h,b) \<in> B \<and> r \<in> R \<longrightarrow> (h, dissemble_arg args (b,r)) \<in> A)"
 
-lemma [\<nu>intro]: "Arguments \<tort_lbrace>r \<tycolon> R\<heavy_comma> \<^bold>h\<^bold>e\<^bold>a\<^bold>p H\<tort_rbrace> \<tort_lbrace>Void\<heavy_comma> \<^bold>h\<^bold>e\<^bold>a\<^bold>p H\<tort_rbrace> \<tort_lbrace>r \<tycolon> R\<tort_rbrace> no_argument"
+lemma [\<nu>intro 1]: "Arguments \<tort_lbrace>r \<tycolon> R\<heavy_comma> \<^bold>h\<^bold>e\<^bold>a\<^bold>p H\<tort_rbrace> \<tort_lbrace>Void\<heavy_comma> \<^bold>h\<^bold>e\<^bold>a\<^bold>p H\<tort_rbrace> \<tort_lbrace>r \<tycolon> R\<tort_rbrace> no_argument"
   unfolding no_argument_def Arguments_def by simp
-lemma [\<nu>intro]: "Arguments \<tort_lbrace>a \<tycolon> A\<heavy_comma> \<^bold>h\<^bold>e\<^bold>a\<^bold>p H\<tort_rbrace> \<tort_lbrace>b \<tycolon> B\<heavy_comma> \<^bold>h\<^bold>e\<^bold>a\<^bold>p H\<tort_rbrace> R args
+lemma [\<nu>intro 1]: "Arguments \<tort_lbrace>a \<tycolon> A\<heavy_comma> \<^bold>h\<^bold>e\<^bold>a\<^bold>p H\<tort_rbrace> \<tort_lbrace>b \<tycolon> B\<heavy_comma> \<^bold>h\<^bold>e\<^bold>a\<^bold>p H\<tort_rbrace> R args
   \<Longrightarrow> Arguments \<tort_lbrace>a \<tycolon> A\<heavy_comma> x \<tycolon> X\<heavy_comma> \<^bold>h\<^bold>e\<^bold>a\<^bold>p H\<tort_rbrace> \<tort_lbrace>b \<tycolon> B\<heavy_comma> x \<tycolon> X\<heavy_comma> \<^bold>h\<^bold>e\<^bold>a\<^bold>p H\<tort_rbrace> R (and_argument args TYPE('xp))"
   for X :: "('xp::lrep, 'x) \<nu>" unfolding and_argument_def Arguments_def by (cases args) (auto 0 3 split: prod.split) 
-lemma [\<nu>intro]: "(\<And>c. Arguments \<tort_lbrace>x c \<tycolon> T c\<tort_rbrace> \<tort_lbrace>x' c \<tycolon> T' c\<tort_rbrace> R arg) \<Longrightarrow> Arguments \<tort_lbrace>x \<tycolon> ExNu T\<tort_rbrace> \<tort_lbrace>x' \<tycolon> ExNu T'\<tort_rbrace> R arg"
+lemma [\<nu>intro 1]: "(\<And>c. Arguments \<tort_lbrace>x c \<tycolon> T c\<tort_rbrace> \<tort_lbrace>x' c \<tycolon> T' c\<tort_rbrace> R arg) \<Longrightarrow> Arguments \<tort_lbrace>x \<tycolon> ExNu T\<tort_rbrace> \<tort_lbrace>x' \<tycolon> ExNu T'\<tort_rbrace> R arg"
   unfolding Arguments_def by auto blast
 
 definition op_call :: " ('r1, 'a \<times> 'r2) argument_types \<Rightarrow> ('r3, 'b \<times> 'r2) argument_types \<Rightarrow> ('a \<longmapsto> 'b) \<Rightarrow> ('r1 \<longmapsto> 'r3)"
@@ -947,15 +1110,15 @@ translations "\<^bold>i\<^bold>n\<^bold>d\<^bold>e\<^bold>x idx \<blangle> x \<t
   "\<^bold>i\<^bold>n\<^bold>d\<^bold>e\<^bold>x idx \<blangle> X \<^bold>@ A \<longmapsto> Y \<^bold>@ b \<tycolon> B \<brangle>" \<rightleftharpoons> "\<^bold>i\<^bold>n\<^bold>d\<^bold>e\<^bold>x idx \<blangle> X \<^bold>@ A  \<longmapsto> Y \<^bold>@ \<tort_lbrace>b  \<tycolon> B\<tort_rbrace> \<brangle>"
 
 
-lemma index_here_getter[\<nu>intro]: "\<^bold>i\<^bold>n\<^bold>d\<^bold>e\<^bold>x index_here \<blangle> A \<^bold>@ A \<brangle>"
+lemma index_here_getter[\<nu>intro 1]: "\<^bold>i\<^bold>n\<^bold>d\<^bold>e\<^bold>x index_here \<blangle> A \<^bold>@ A \<brangle>"
   unfolding \<nu>index_def  index_here_def by auto
-lemma index_here_mapper[\<nu>intro]: "\<^bold>i\<^bold>n\<^bold>d\<^bold>e\<^bold>x index_here \<blangle> A \<^bold>@ A \<longmapsto> B \<^bold>@ B \<brangle>"
+lemma index_here_mapper[\<nu>intro 1]: "\<^bold>i\<^bold>n\<^bold>d\<^bold>e\<^bold>x index_here \<blangle> A \<^bold>@ A \<longmapsto> B \<^bold>@ B \<brangle>"
   unfolding \<nu>index_def  index_here_def by auto
 (* lemma index_left_getter[\<nu>intro]: "\<^bold>i\<^bold>n\<^bold>d\<^bold>e\<^bold>x f \<blangle> X \<^bold>@ A \<brangle> \<Longrightarrow> \<^bold>i\<^bold>n\<^bold>d\<^bold>e\<^bold>x index_left f \<blangle> X \<^bold>@ (A \<^bold>a\<^bold>n\<^bold>d R) \<brangle>"
   unfolding \<nu>index_def index_left_def by (cases f) auto
 lemma index_right_getter[\<nu>intro]: "\<^bold>i\<^bold>n\<^bold>d\<^bold>e\<^bold>x f \<blangle> X \<^bold>@ A \<brangle> \<Longrightarrow> \<^bold>i\<^bold>n\<^bold>d\<^bold>e\<^bold>x index_right f \<blangle> X \<^bold>@ (L \<^bold>a\<^bold>n\<^bold>d A) \<brangle>"
   unfolding \<nu>index_def index_right_def by (cases f) auto *)
-lemma index_stack_getter[\<nu>intro]: "\<^bold>i\<^bold>n\<^bold>d\<^bold>e\<^bold>x f \<blangle> X \<^bold>@ a \<tycolon> A \<brangle> \<Longrightarrow> \<^bold>i\<^bold>n\<^bold>d\<^bold>e\<^bold>x index_right f \<blangle> X \<^bold>@ (a \<tycolon> A\<heavy_comma> x \<tycolon> N) \<brangle>"
+lemma index_stack_getter[\<nu>intro 1]: "\<^bold>i\<^bold>n\<^bold>d\<^bold>e\<^bold>x f \<blangle> X \<^bold>@ a \<tycolon> A \<brangle> \<Longrightarrow> \<^bold>i\<^bold>n\<^bold>d\<^bold>e\<^bold>x index_right f \<blangle> X \<^bold>@ (a \<tycolon> A\<heavy_comma> x \<tycolon> N) \<brangle>"
   unfolding \<nu>index_def index_right_def by (cases f) auto
 (* lemma index_left_mapper[\<nu>intro]:
     "\<^bold>i\<^bold>n\<^bold>d\<^bold>e\<^bold>x f \<blangle> X \<^bold>@ A \<longmapsto> Y \<^bold>@ B\<brangle> \<Longrightarrow> \<^bold>i\<^bold>n\<^bold>d\<^bold>e\<^bold>x index_left f \<blangle> X \<^bold>@ (A \<^bold>a\<^bold>n\<^bold>d R) \<longmapsto> Y \<^bold>@ (B \<^bold>a\<^bold>n\<^bold>d R) \<brangle>"
@@ -963,7 +1126,7 @@ lemma index_stack_getter[\<nu>intro]: "\<^bold>i\<^bold>n\<^bold>d\<^bold>e\<^bo
 lemma index_right_mapper[\<nu>intro]:
     "\<^bold>i\<^bold>n\<^bold>d\<^bold>e\<^bold>x f \<blangle> X \<^bold>@ A \<longmapsto> Y \<^bold>@ B\<brangle> \<Longrightarrow> \<^bold>i\<^bold>n\<^bold>d\<^bold>e\<^bold>x index_right f \<blangle> X \<^bold>@ (L \<^bold>a\<^bold>n\<^bold>d A) \<longmapsto> Y \<^bold>@ (L \<^bold>a\<^bold>n\<^bold>d B) \<brangle>"
   unfolding \<nu>index_def index_right_def by (cases f) auto *)
-lemma index_stack_mapper[\<nu>intro]:
+lemma index_stack_mapper[\<nu>intro 1]:
     "\<^bold>i\<^bold>n\<^bold>d\<^bold>e\<^bold>x f \<blangle> X \<^bold>@ a \<tycolon> A \<longmapsto> Y \<^bold>@ b \<tycolon> B\<brangle> \<Longrightarrow> \<^bold>i\<^bold>n\<^bold>d\<^bold>e\<^bold>x index_right f \<blangle> X \<^bold>@ (a \<tycolon> A\<heavy_comma> N) \<longmapsto> Y \<^bold>@ (b \<tycolon> B\<heavy_comma> N) \<brangle>"
   unfolding \<nu>index_def index_right_def by (cases f) auto
 
@@ -1119,9 +1282,8 @@ attribute_setup \<nu>process = \<open>Scan.lift (Parse.$$$ "(" |-- Parse.name_po
   \<open>Evaluate the \<nu>-system process or the process of the given processor on the target theorem\<close>
 
 method_setup \<nu>reason = \<open>let open Scan Parse in
-  (succeed NONE ||
-  (Attrib.thms -- option (lift ($$$ "(") |-- Attrib.thms --| lift ($$$ ")") -- (lift ($$$ "(") |-- Attrib.thms --| lift ($$$ ")"))) >> SOME))
-  >> (fn ths => fn ctx => Method.METHOD (fn th2 => NuSys.auto_resolve (@{print} ths) th2 ctx))
+  (succeed [] || Scan.repeat (Attrib.thms -- Scan.lift Parse.int)) >> (fn ths => fn ctx =>
+  Method.SIMPLE_METHOD (Nu_Reasoner.reason_tac (Nu_Reasoner.add_intro_rules ths ctx)))
 end\<close>
 
 ML \<open>
@@ -1337,7 +1499,7 @@ subsubsection \<open>Sub-procedure\<close>
 
 \<nu>processor end_sub_procedure 7000 \<open>\<^bold>c\<^bold>u\<^bold>r\<^bold>r\<^bold>e\<^bold>n\<^bold>t blk \<^bold>r\<^bold>e\<^bold>s\<^bold>u\<^bold>l\<^bold>t\<^bold>s \<^bold>i\<^bold>n T\<close> \<open>let open Parse Scan in fn ctx => fn meta =>
   $$$ "\<medium_right_bracket>" >> (fn x => fn () =>
-  (@{print} x; raise Process_State_Call' (meta, NuToplevel.end_block_cmd true))
+  raise Process_State_Call' (meta, NuToplevel.end_block_cmd true)
 ) end\<close>
 
 (*
@@ -1362,9 +1524,12 @@ subsection \<open>Simplifiers & Resonings\<close>
 \<nu>processor \<nu>simplifier 40 \<open>\<^bold>c\<^bold>u\<^bold>r\<^bold>r\<^bold>e\<^bold>n\<^bold>t blk \<^bold>r\<^bold>e\<^bold>s\<^bold>u\<^bold>l\<^bold>t\<^bold>s \<^bold>i\<^bold>n T\<close>  \<open>NuProcessors.simplifier []\<close>
 (* \<nu>processor \<nu>simplifier_final 9999 \<open>PROP P\<close>  \<open>NuProcessors.simplifier []\<close> *)
 
-\<nu>processor \<nu>resolver 1000 \<open>PROP P \<Longrightarrow> PROP Q\<close> \<open>fn ctx => fn meta => Scan.succeed (fn _ =>
-  NuSys.auto_resolve_rule NONE [] (NuSys.load_specthm meta ctx) meta
-    handle NuSys.ReasoningFail _ => raise Bypass NONE)\<close>
+\<nu>processor \<nu>reason 1000 \<open>PROP P \<Longrightarrow> PROP Q\<close> \<open>fn ctx => fn meta => Scan.succeed (fn _ =>
+  let open NuBasics
+    val meta' = elim_SPEC meta
+      |> apfst (Nu_Reasoner.reason (NuSys.load_specthm meta ctx))
+      |> intro_SPEC
+  in if Thm.prop_of meta = Thm.prop_of meta' then raise Bypass (SOME meta') else meta' end)\<close>
 
 subsection \<open>Literal operations\<close>
 
@@ -1372,18 +1537,6 @@ subsection \<open>Literal operations\<close>
   let val term = Syntax.read_term ctx term |> Thm.cterm_of ctx |> Simplifier.rewrite ctx |> Thm.rhs_of
         val ctx = NuSys.load_specthm meta ctx
   in NuSys.auto_construct ctx term meta end)\<close>
-
-\<nu>processor literal_number 9500\<open>\<^bold>c\<^bold>u\<^bold>r\<^bold>r\<^bold>e\<^bold>n\<^bold>t blk \<^bold>r\<^bold>e\<^bold>s\<^bold>u\<^bold>l\<^bold>t\<^bold>s \<^bold>i\<^bold>n T\<close> \<open>fn ctx => fn meta => Parse.number >> (fn num => fn _ =>
-  let open NuBasics
-    val num = Syntax.parse_term ctx num
-    fun mk term = mk_nuTy (num, term) |> Syntax.check_term ctx |> Thm.cterm_of ctx
-    val term = ((stack_of_meta meta |> hd |> #2 |> mk)
-      handle TERM _ => mk @{term \<open>\<nat>[32]\<close>}
-        | ERROR _ => mk @{term \<open>\<nat>[32]\<close>}) |> @{print}
-    val ctx = NuSys.load_specthm meta ctx
-  in NuSys.auto_construct ctx term meta  end)
-\<close>
-
 
 section \<open>Mechanism III\<close>
 
@@ -1427,5 +1580,11 @@ let open Parse Scan NuHelp NuBasics in
     >> (fn ((((vars, stack_schema), heap_schema)), always) => fn _ =>
       NuVariablesTag.variables_tag_pattern_match (flat vars) stack_schema heap_schema always ctx meta)
 end\<close>
+
+subsection \<open>Auto Reasoners\<close>
+
+ML_file "library/reasoners.ML"
+
+\<nu>reasoner \<open>\<^bold>p\<^bold>r\<^bold>e\<^bold>m\<^bold>i\<^bold>s\<^bold>e P\<close> 0 = \<open>Nu_Reasoners.premise_tac\<close>
 
 end
