NuBasicAbstractors.thy
@@ -92,14 +92,14 @@ lemma [elim,\<nu>elim]: "a \<R_arr_tail> xs \<ratio> Array' N \<Longrightarrow> 
   unfolding Inhabited_def[of "\<tort_lbrace>a \<R_arr_tail> xs \<tycolon> Array' N\<tort_rbrace>"]
   by (cases a) (auto simp add: lrep_exps pred_option_def list_all2_conv_all_nth)
 
-lemma Array'_to_Ref_\<nu>proc[\<nu>intro]:
+lemma Array'_to_Ref_\<nu>proc[\<nu>intro -300]:
  "\<^bold>p\<^bold>r\<^bold>e\<^bold>m\<^bold>i\<^bold>s\<^bold>e i < length xs \<Longrightarrow> \<^bold>p\<^bold>r\<^bold>e\<^bold>m\<^bold>i\<^bold>s\<^bold>e (xs ! i) \<noteq> None \<Longrightarrow>
   \<^bold>d\<^bold>e\<^bold>s\<^bold>t \<^bold>c\<^bold>a\<^bold>s\<^bold>t a \<R_arr_tail> xs \<tycolon> Array' N \<longmapsto> a \<R_arr_tail> xs[i := None] \<tycolon> Array' N \<heavy_asterisk> (a ||+ i) \<R_arr_tail> the (xs ! i) \<tycolon> Ref N"
   unfolding Dest_def Cast_def Heap_Delimiter_def
   apply (cases a) apply auto apply (rule heap_split_by_addr_set[of _  _ "-{a ||+ i}"])
   by (auto simp add: pred_option_def Ball_def nth_list_update)
 
-lemma [\<nu>intro]:
+lemma [\<nu>intro -1]:
   "\<^bold>p\<^bold>r\<^bold>e\<^bold>m\<^bold>i\<^bold>s\<^bold>e i < length xs \<Longrightarrow>
   \<^bold>i\<^bold>n\<^bold>t\<^bold>r\<^bold>o \<^bold>c\<^bold>a\<^bold>s\<^bold>t a \<R_arr_tail> xs[i := None] \<tycolon> Array' N \<heavy_asterisk> (a ||+ i) \<R_arr_tail> y \<tycolon> Ref N \<longmapsto> a \<R_arr_tail> xs[i := Some y] \<tycolon> Array' N"
   unfolding Intro_def Cast_def Heap_Delimiter_def
@@ -136,7 +136,7 @@ lemma [elim,\<nu>elim]: "a \<R_arr_tail> xs \<ratio> Array N \<Longrightarrow> (
   unfolding Array_def
   by (cases a) (auto simp add: lrep_exps list_all2_conv_all_nth)
 
-lemma [THEN cast_trans, simplified, \<nu>intro]:
+lemma [THEN cast_trans, simplified, \<nu>intro -3]:
   "\<^bold>c\<^bold>a\<^bold>s\<^bold>t a \<R_arr_tail> xs \<tycolon> Array N \<longmapsto> a \<R_arr_tail> map Some xs \<tycolon> Array' N"
   unfolding Cast_def Array_def by (cases a) auto
 
@@ -147,9 +147,9 @@ lemma [simp]: "i < length l \<Longrightarrow> (mapSome l) [i := Some v] = mapSom
 lemma [simp]: "i < length l \<Longrightarrow> the (mapSome l ! i) = l ! i" unfolding mapSome_def by auto
 
 
-lemma [\<nu>intro]: "\<^bold>p\<^bold>r\<^bold>e\<^bold>m\<^bold>i\<^bold>s\<^bold>e xs' = mapSome xs2 \<Longrightarrow> \<^bold>i\<^bold>n\<^bold>t\<^bold>r\<^bold>o \<^bold>c\<^bold>a\<^bold>s\<^bold>t  a \<R_arr_tail> xs' \<tycolon> Array' N \<longmapsto> a \<R_arr_tail> xs2 \<tycolon> Array N"
+lemma [\<nu>intro -1]: "\<^bold>p\<^bold>r\<^bold>e\<^bold>m\<^bold>i\<^bold>s\<^bold>e xs' = mapSome xs2 \<Longrightarrow> \<^bold>i\<^bold>n\<^bold>t\<^bold>r\<^bold>o \<^bold>c\<^bold>a\<^bold>s\<^bold>t  a \<R_arr_tail> xs' \<tycolon> Array' N \<longmapsto> a \<R_arr_tail> xs2 \<tycolon> Array N"
   unfolding Cast_def Intro_def Array_def by (cases a) (auto simp add: pred_option_def Ball_def)
-lemma [\<nu>intro]: "\<^bold>d\<^bold>e\<^bold>s\<^bold>t \<^bold>c\<^bold>a\<^bold>s\<^bold>t a \<R_arr_tail> xs \<tycolon> Array N \<longmapsto> a \<R_arr_tail> mapSome xs \<tycolon> Array' N"
+lemma [\<nu>intro -300]: "\<^bold>d\<^bold>e\<^bold>s\<^bold>t \<^bold>c\<^bold>a\<^bold>s\<^bold>t a \<R_arr_tail> xs \<tycolon> Array N \<longmapsto> a \<R_arr_tail> mapSome xs \<tycolon> Array' N"
   unfolding Cast_def Dest_def Array_def by (cases a) (auto simp add: pred_option_def Ball_def)
 
 
