NuInstructions.thy
@@ -1,5 +1,5 @@
 theory NuInstructions
-  imports NuSys NuBasicAbstractors
+  imports NuSys NuBasicAbstractors NuLLReps
   keywords
      "\<up>:" "\<Up>:" "\<down>:" "\<Down>:" "subj" "always" "heap" "--" :: quasi_command
   abbrevs "|^" = "\<up>"
@@ -176,8 +176,7 @@ lemma do_while_\<nu>proc:
 
 
 subsubsection \<open>while\<close>
-
-ML \<open>order_list\<close>
+ML \<open>find_first\<close>
 proc while: \<open>s' \<tycolon> S'\<heavy_comma> \<^bold>h\<^bold>e\<^bold>a\<^bold>p h' \<tycolon> H'\<close> \<longmapsto> \<open>\<exists>* x. (x \<tycolon> S\<heavy_comma> \<^bold>h\<^bold>e\<^bold>a\<^bold>p x \<tycolon> H) \<and>\<^sup>\<nu>\<^sub>a\<^sub>u\<^sub>t\<^sub>o (\<not> cond x)\<close>
   requires [unfolded Variant_Cast_def, simp]: "Variant_Cast (s' \<tycolon> S') (h' \<tycolon> H') vars S H"
     and Cond_\<nu>proc: "\<forall>x. \<^bold>p\<^bold>r\<^bold>o\<^bold>c Cond \<blangle> x \<tycolon> S\<heavy_comma> \<^bold>h\<^bold>e\<^bold>a\<^bold>p x \<tycolon> H \<longmapsto> \<exists>* x'. (x' \<tycolon> S\<heavy_comma> cond x' \<tycolon> \<bool>\<heavy_comma> \<^bold>h\<^bold>e\<^bold>a\<^bold>p x' \<tycolon> H)\<brangle>"
@@ -236,26 +235,26 @@ theorem const_nat_\<nu>proc: "\<^bold>p\<^bold>r\<^bold>o\<^bold>c op_const_int 
 (* theorem const_nat_round_\<nu>proc: "\<^bold>p\<^bold>r\<^bold>o\<^bold>c op_const_int TYPE('w::len) (of_nat n) \<blangle> R \<longmapsto> R \<heavy_comma> n \<tycolon> \<nat>\<^sup>r['w] \<brangle>"
   unfolding \<nu>def op_const_int_def by auto *)
 
-lemma [\<nu>intro]:
+lemma [\<nu>intro 1]:
   "\<^bold>p\<^bold>r\<^bold>e\<^bold>m\<^bold>i\<^bold>s\<^bold>e (numeral x :: nat) < 2^LENGTH('w) \<Longrightarrow>
    \<^bold>c\<^bold>o\<^bold>n\<^bold>s\<^bold>t\<^bold>r\<^bold>u\<^bold>c\<^bold>t ((numeral x) \<tycolon> \<nat>['w]) \<^bold>b\<^bold>y \<^bold>p\<^bold>r\<^bold>o\<^bold>c op_const_int TYPE('w::len) (Word.of_nat (numeral x)) \<blangle> R\<heavy_comma> \<^bold>h\<^bold>e\<^bold>a\<^bold>p H \<longmapsto> R \<heavy_comma> (numeral x) \<tycolon> \<nat>['w]\<heavy_comma> \<^bold>h\<^bold>e\<^bold>a\<^bold>p H \<brangle>"
   unfolding op_const_int_def \<nu>def including show_more1 apply auto by (metis mod_if unat_bintrunc unat_numeral)
   \<comment> \<open>Only literal number could be constructed automatically\<close>
-lemma [\<nu>intro]:
+lemma [\<nu>intro 1]:
   "\<^bold>c\<^bold>o\<^bold>n\<^bold>s\<^bold>t\<^bold>r\<^bold>u\<^bold>c\<^bold>t (0 \<tycolon> \<nat>['w]) \<^bold>b\<^bold>y \<^bold>p\<^bold>r\<^bold>o\<^bold>c op_const_int TYPE('w::len) 0 \<blangle> R\<heavy_comma> \<^bold>h\<^bold>e\<^bold>a\<^bold>p H \<longmapsto> R \<heavy_comma> 0 \<tycolon> \<nat>['w]\<heavy_comma> \<^bold>h\<^bold>e\<^bold>a\<^bold>p H \<brangle>"
   unfolding AutoConstruct_def using const_nat_\<nu>proc by (metis unat_0) 
-lemma [\<nu>intro]:
+lemma [\<nu>intro 1]:
   "\<^bold>c\<^bold>o\<^bold>n\<^bold>s\<^bold>t\<^bold>r\<^bold>u\<^bold>c\<^bold>t (1 \<tycolon> \<nat>['w]) \<^bold>b\<^bold>y \<^bold>p\<^bold>r\<^bold>o\<^bold>c op_const_int TYPE('w::len) 1 \<blangle> R\<heavy_comma> \<^bold>h\<^bold>e\<^bold>a\<^bold>p H \<longmapsto> R\<heavy_comma> 1 \<tycolon> \<nat>['w]\<heavy_comma> \<^bold>h\<^bold>e\<^bold>a\<^bold>p H \<brangle>"
   unfolding AutoConstruct_def using const_nat_\<nu>proc by (metis unat_1)
 
-lemma [\<nu>intro]:
+lemma [\<nu>intro 1]:
   "\<^bold>p\<^bold>r\<^bold>e\<^bold>m\<^bold>i\<^bold>s\<^bold>e (numeral x :: nat) < 2^LENGTH('w) \<Longrightarrow>
    \<^bold>c\<^bold>o\<^bold>n\<^bold>s\<^bold>t\<^bold>r\<^bold>u\<^bold>c\<^bold>t ((numeral x) \<tycolon> \<nat>\<^sup>r['w]) \<^bold>b\<^bold>y \<^bold>p\<^bold>r\<^bold>o\<^bold>c op_const_int TYPE('w::len) (Word.of_nat (numeral x)) \<blangle> R\<heavy_comma> \<^bold>h\<^bold>e\<^bold>a\<^bold>p H \<longmapsto> R\<heavy_comma> (numeral x) \<tycolon> \<nat>\<^sup>r['w]\<heavy_comma> \<^bold>h\<^bold>e\<^bold>a\<^bold>p H \<brangle>"
   unfolding op_const_int_def \<nu>def including show_more1 by auto
-lemma [\<nu>intro]:
+lemma [\<nu>intro 1]:
   "\<^bold>c\<^bold>o\<^bold>n\<^bold>s\<^bold>t\<^bold>r\<^bold>u\<^bold>c\<^bold>t (0 \<tycolon> \<nat>\<^sup>r['w]) \<^bold>b\<^bold>y \<^bold>p\<^bold>r\<^bold>o\<^bold>c op_const_int TYPE('w::len) 0 \<blangle> R\<heavy_comma> \<^bold>h\<^bold>e\<^bold>a\<^bold>p H \<longmapsto> R\<heavy_comma> 0 \<tycolon> \<nat>\<^sup>r['w]\<heavy_comma> \<^bold>h\<^bold>e\<^bold>a\<^bold>p H \<brangle>"
   unfolding op_const_int_def \<nu>def including show_more1 by auto
-lemma [\<nu>intro]:
+lemma [\<nu>intro 1]:
   "\<^bold>c\<^bold>o\<^bold>n\<^bold>s\<^bold>t\<^bold>r\<^bold>u\<^bold>c\<^bold>t (1 \<tycolon> \<nat>\<^sup>r['w]) \<^bold>b\<^bold>y \<^bold>p\<^bold>r\<^bold>o\<^bold>c op_const_int TYPE('w::len) 1 \<blangle> R\<heavy_comma> \<^bold>h\<^bold>e\<^bold>a\<^bold>p H \<longmapsto> R\<heavy_comma> 1 \<tycolon> \<nat>\<^sup>r['w]\<heavy_comma> \<^bold>h\<^bold>e\<^bold>a\<^bold>p H \<brangle>"
   unfolding op_const_int_def \<nu>def including show_more1 by auto
 
@@ -575,25 +574,5 @@ thm pair_forall
 thm recursive_func_help_1
 thm NuAddition_anti_auto
 
-ML \<open>try\<close>
-rec_proc Fib: \<open>i \<tycolon> \<nat>[32]\<heavy_comma> (j::int) \<tycolon> X\<close> \<longmapsto> \<open>fib i \<tycolon> \<nat>[32]\<heavy_comma> j \<tycolon> X\<close> var i
-  premises [used]: \<open>0 < i\<close>
-  \<bullet> Fib 
-\<nu>debug thm Fib_\<nu>proc
-  finish
-thm Fib_\<nu>compilation
-thm rename_proc
-
-
-ML \<open>Thm.intro_rules\<close>
-ML \<open>Thmtab.lookup\<close>
-thm apply_proc_conv
-proc test: \<open>R\<heavy_comma> i \<tycolon> \<nat>[32]\<close> \<longmapsto> \<open>R\<heavy_comma> 0 \<tycolon> \<nat>[32]\<close>
-  \<bullet> until i subj \<open>0 < i\<close> \<medium_left_bracket> \<bullet> \<rightarrow> i i 1 -
-  \<bullet> 0 i <
-  thm decorated_All_def[symmetric]
-  \<medium_left_bracket>  \<nu>debug note that 
-
-  thm XXXX
 
 end
